Some progress on Cryptol->Coq theory.

Coq/EC/CryptolToCoq_equiv.v
@@ -31,51 +31,24 @@ From Bits Require Import operations.properties.
 From Bits Require Import spec.properties.
 
 (*
-Axioms on which the main proof depends. If you prove something in this file, remove it from the list. 
+Require Import CryptolToCoq.SAWCoreBitvectorsZifyU64.
+*)
 
+(*
+Axioms on which the main proof depend. If you prove something in this file, remove it from the list. 
 
-toList_reverse_cons_eq
-  : forall (A : Type) (inh : Inhabited A) (n : nat) (ls : Vec n A) (a : A),
-    to_list (reverse (S n) A (cons A a n ls)) = to_list (reverse n A ls) ++ [a]
-toList_drop_equiv
-  : forall (A : Type) (inh : Inhabited A) (n1 n2 : Nat) (ls : Vec (addNat n1 n2) A),
-    to_list (drop A n1 n2 ls) = skipn n1 (to_list ls)
-toList_append_equiv
-  : forall (A : Type) (inh : Inhabited A) (n m : nat) (v1 : Vec n A) (v2 : Vec m A),
-    to_list (append n m A v1 v2) = to_list v1 ++ to_list v2
-ssr_double_even : forall n : nat, Nat.even (ssrnat.double n) = true
-ssr_addn_even : forall n1 n2 : nat, Nat.even n1 = true -> Nat.even n2 = true -> Nat.even (ssrnat.addn n1 n2) = true
-shiftR_false_0 : forall n1 n2 : nat, shiftR n1 bool false (replicate n1 bool false) n2 = replicate n1 bool false
-shiftR_all_nonneg
-  : forall (n1 : nat) (v : bitvector n1),
-    (0 <= sbvToInt n1 v)%Z -> shiftR n1 bool false v (Nat.pred n1) = replicate n1 bool false
-shiftR_all_neg
-  : forall (n1 : nat) (v : bitvector n1), (sbvToInt n1 v < 0)%Z -> shiftR n1 bool false v (Nat.pred n1) = intToBv n1 1
-shiftL_shiftL
-  : forall (A : Type) (n : nat) (b : A) (v : t A n) (n1 n2 : nat),
-    shiftL n A b (shiftL n A b v n1) n2 = shiftL n A b v (n1 + n2)
 sbvToInt_sign_extend_equiv
   : forall (n1 : Nat) (n2 : nat) (x : bitvector n1),
     sbvToInt (addNat n2 n1)
-      (append n2 n1 Bool
-         (if sawAt n1 Bool x 0%nat
-          then ecCompl (bitvector n2) (PLogicWord n2) (ecZero (bitvector n2) (intToBv n2 0))
-          else ecZero (bitvector n2) (intToBv n2 0)) x) = sbvToInt n1 x
-sbvToInt_shiftL_1_equiv
-  : forall n s : nat,
-    n > 0 -> s < Nat.pred n -> sbvToInt n (shiftL n bool false (intToBv n 1) s) = BinInt.Z.shiftl 1 (BinInt.Z.of_nat s)
-sbvToInt_replicate_0 : forall n : Nat, sbvToInt n (replicate n bool false) = 0%Z
-sbvToInt_nz_nth : forall (n : nat) (v : Vec n bool) (n' : nat) (nlt : n' < n), nth_order v nlt = true -> sbvToInt n v <> 0%Z
-sbvToInt_neg_sign_bit_set
-  : forall (n : nat) (b2 : bitvector n) (ltpf : 0 < n), (sbvToInt n b2 < 0)%Z -> nth_order b2 ltpf = true
-sbvToInt_intToBv_id
-  : forall (n : nat) (v : Z),
-    (- 2 ^ BinInt.Z.of_nat (Nat.pred n) <= v < 2 ^ BinInt.Z.of_nat (Nat.pred n))%Z -> sbvToInt n (intToBv n v) = v
+      (append n2 n1 Bool (if sawAt n1 Bool x 0%nat then ecCompl (bitvector n2) (PLogicWord n2) (ecZero (bitvector n2) (intToBv n2 0)) else ecZero (bitvector n2) (intToBv n2 0)) x) =
+    sbvToInt n1 x
+
+
+sbvToInt_intToBv_id : forall (n : nat) (v : Z), (- 2 ^ BinInt.Z.of_nat (Nat.pred n) <= v < 2 ^ BinInt.Z.of_nat (Nat.pred n))%Z -> sbvToInt n (intToBv n v) = v
 sbvToInt_drop_equiv_h
   : forall (n1 : Nat) (n2 : nat) (x : bitvector (addNat n1 (S n2))),
-    (- 2 ^ BinInt.Z.of_nat n2 <= sbvToInt (addNat n1 (S n2)) x < 2 ^ BinInt.Z.of_nat n2)%Z ->
-    spec.toZ (bvToBITS (drop Bool n1 (S n2) x)) = sbvToInt (addNat n1 (S n2)) x
-sbvToInt_bvToInt_id : forall (n : Nat) (x : bitvector n), intToBv n (sbvToInt n x) = x
+    (- 2 ^ BinInt.Z.of_nat n2 <= sbvToInt (addNat n1 (S n2)) x < 2 ^ BinInt.Z.of_nat n2)%Z -> spec.toZ (bvToBITS (drop Bool n1 (S n2) x)) = sbvToInt (addNat n1 (S n2)) x
+sbvToInt_bvToInt_id : forall (n : nat) (x : bitvector n), n > 0 -> intToBv n (sbvToInt n x) = x
 sbvToInt_bvSub_equiv
   : forall (n : nat) (v1 v2 : bitvector n),
     n > 1 ->
@@ -83,120 +56,72 @@ sbvToInt_bvSub_equiv
     (- 2 ^ BinInt.Z.of_nat (Nat.pred (Nat.pred n)) <= sbvToInt n v2 < 2 ^ BinInt.Z.of_nat (Nat.pred (Nat.pred n)))%Z ->
     sbvToInt n (bvSub n v1 v2) = (sbvToInt n v1 - sbvToInt n v2)%Z
 sbvToInt_bvNeg_equiv : forall (n : Nat) (v : bitvector n), sbvToInt n (bvNeg n v) = (- sbvToInt n v)%Z
-sbvToInt_0_replicate : forall (n : Nat) (b2 : bitvector n), sbvToInt n b2 = 0%Z -> b2 = replicate n bool false
-sawAt_nth_order_equiv
-  : forall (A : Type) (inh : Inhabited A) (n1 n2 : nat) (v : Vec n1 A) (ltpf : n2 < n1), sawAt n1 A v n2 = nth_order v ltpf
-sawAt_3_equiv
-  : forall (A : Type) (inh : Inhabited A) (v : t A 3),
-    cons A (sawAt 3 A v 0%nat) 2 (cons A (sawAt 3 A v 1%nat) 1 (cons A (sawAt 3 A v 2) 0 (nil A))) = v
-rep_false_eq_int_bv : forall n : Nat, replicate n bool false = intToBv n 0
-nth_order_shiftR_all_eq
-  : forall (A : Type) (n2 len : nat) (v : Vec len A) (nlt : n2 < len) (zlt : 0 < len) (a : A),
-    nth_order (shiftR len A a v n2) nlt = nth_order v zlt
+sbvToInt_0_replicate : forall (n : Nat) (b2 : bitvector n), sbvToInt n b2 = 0%Z -> b2 = replicate n bool 0%bool
+sawAt_nth_order_equiv : forall (A : Type) (inh : Inhabited A) (n1 n2 : nat) (v : Vec n1 A) (ltpf : n2 < n1), sawAt n1 A v n2 = nth_order v ltpf
+sawAt_3_equiv : forall (A : Type) (inh : Inhabited A) (v : t A 3), cons A (sawAt 3 A v 0%nat) 2 (cons A (sawAt 3 A v 1%nat) 1 (cons A (sawAt 3 A v 2) 0 (nil A))) = v
+rep_false_eq_int_bv : forall n : Nat, replicate n bool 0%bool = intToBv n 0
+nth_order_shiftR_all_eq : forall (A : Type) (n2 len : nat) (v : Vec len A) (nlt : n2 < len) (zlt : 0 < len) (a : A), nth_order (shiftR len A a v n2) nlt = nth_order v zlt
 nth_order_drop_eq
-  : forall (A : Type) (inh : Inhabited A) (n1 n2 : Nat) (v : Vec (addNat n1 n2) A) (n' : Nat)
-      (lt1 : addNat n1 n' < addNat n1 n2) (lt2 : n' < n2), nth_order (drop A n1 n2 v) lt2 = nth_order v lt1
-nth_order_bvAnd_l_eq
-  : forall (n : nat) (v : bitvector n) (n' : nat) (plt : n' < n),
-    n' < Nat.pred n -> nth_order (bvAnd n v (intToBv n 1)) plt = false
-nth_order_bvAnd_eq
-  : forall (n : nat) (v : bitvector n) (plt : Nat.pred n < n), nth_order (bvAnd n v (intToBv n 1)) plt = nth_order v plt
+  : forall (A : Type) (inh : Inhabited A) (n1 n2 : Nat) (v : Vec (addNat n1 n2) A) (n' : Nat) (lt1 : addNat n1 n' < addNat n1 n2) (lt2 : n' < n2),
+    nth_order (drop A n1 n2 v) lt2 = nth_order v lt1
+nth_order_bvAnd_l_eq : forall (n : nat) (v : bitvector n) (n' : nat) (plt : n' < n), n' < Nat.pred n -> nth_order (bvAnd n v (intToBv n 1)) plt = 0%bool
+nth_order_bvAnd_eq : forall (n : nat) (v : bitvector n) (plt : Nat.pred n < n), nth_order (bvAnd n v (intToBv n 1)) plt = nth_order v plt
 nth_order_append_l_eq
-  : forall (A : Type) (inh : Inhabited A) (n1 : nat) (v1 : Vec n1 A) (n2 : nat) (v2 : Vec n2 A) (n' : nat)
-      (nlt2 : n' < addNat n2 n1) (nlt1 : n' < n2), nth_order (append n2 n1 A v2 v1) nlt2 = nth_order v2 nlt1
+  : forall (A : Type) (inh : Inhabited A) (n1 : nat) (v1 : Vec n1 A) (n2 : nat) (v2 : Vec n2 A) (n' : nat) (nlt2 : n' < addNat n2 n1) (nlt1 : n' < n2),
+    nth_order (append n2 n1 A v2 v1) nlt2 = nth_order v2 nlt1
 nth_order_append_eq
-  : forall (A : Type) (inh : Inhabited A) (n1 : nat) (v1 : Vec n1 A) (n2 : nat) (v2 : Vec n2 A) (n' : Nat)
-      (nlt2 : addNat n' n2 < addNat n2 n1) (nlt1 : n' < n1), nth_order (append n2 n1 A v2 v1) nlt2 = nth_order v1 nlt1
-nth_order_0 : forall (n1 n2 : nat) (nlt : n2 < n1), nth_order (intToBv n1 0) nlt = false
-intToBv_eq_pos
-  : forall (n : nat) (x y : Z),
-    (0 <= x < 2 ^ BinInt.Z.of_nat n)%Z -> (0 <= y < 2 ^ BinInt.Z.of_nat n)%Z -> intToBv n x = intToBv n y -> x = y
+  : forall (A : Type) (inh : Inhabited A) (n1 : nat) (v1 : Vec n1 A) (n2 : nat) (v2 : Vec n2 A) (n' : Nat) (nlt2 : addNat n' n2 < addNat n2 n1) (nlt1 : n' < n1),
+    nth_order (append n2 n1 A v2 v1) nlt2 = nth_order v1 nlt1
+nth_order_0 : forall (n1 n2 : nat) (nlt : n2 < n1), nth_order (intToBv n1 0) nlt = 0%bool
+intToBv_eq_pos : forall (n : nat) (x y : Z), (0 <= x < 2 ^ BinInt.Z.of_nat n)%Z -> (0 <= y < 2 ^ BinInt.Z.of_nat n)%Z -> intToBv n x = intToBv n y -> x = y
 intToBv_add_equiv : forall (n : Nat) (x y : Z), intToBv n (x + y) = bvAdd n (intToBv n x) (intToBv n y)
-intToBv_0_eq_replicate : forall n : Nat, intToBv n 0 = replicate n bool false
-intToBv_0_S : forall n : nat, intToBv (S n) 0 = cons bool false n (intToBv n 0)
+intToBv_0_eq_replicate : forall n : Nat, intToBv n 0 = replicate n bool 0%bool
+intToBv_0_S : forall n : nat, intToBv (S n) 0 = cons bool 0%bool n (intToBv n 0)
 holds_up_to_3 : forall P : nat -> Prop, P 0%nat -> P 1%nat -> P 2 -> P 3 -> forall n : nat, P n
-foldl_dep_tuple_cons
-  : forall (n : nat) (x : t bool n) (b : bool),
-    foldl_dep bool (fun n0 : Nat => tuple.tuple_of (S n0) bool) n
-      (fun (n0 : Nat) (bs : tuple.tuple_of (S n0) bool) (b0 : bool) => tuple.cons_tuple b0 bs)
-      (tuple.cons_tuple b (tuple.nil_tuple bool)) x =
-    tuple.cons_tuple b
-      (foldl_dep bool (fun n0 : Nat => tuple.tuple_of n0 bool) n
-         (fun (n0 : Nat) (bs : tuple.tuple_of n0 bool) (b0 : bool) => tuple.cons_tuple b0 bs) (tuple.nil_tuple bool) x)
 error : forall a : Type, Inhabited a -> string -> a
 Eqdep.Eq_rect_eq.eq_rect_eq : forall (U : Type) (p : U) (Q : U -> Type) (x : Q p) (h : p = p), x = eq_rect p Q x p h
-ecOr_0_if
-  : forall (n : nat) (x y : bitvector n),
-    ecOr (bitvector n) (PLogicWord n) x y = replicate n bool false ->
-    x = replicate n bool false /\ y = replicate n bool false
-ecNotEq_vec_bv_true
-  : forall (n1 n2 : nat) (v1 v2 : Vec n1 (bitvector n2)),
-    v1 <> v2 -> ecNotEq (Vec n1 (bitvector n2)) (PEqVec n1 (bitvector n2) (PEqWord n2)) v1 v2 = true
-ecNotEq_vec_bv_false
-  : forall (n1 n2 : nat) (v : Vec n1 (bitvector n2)),
-    ecNotEq (Vec n1 (bitvector n2)) (PEqVec n1 (bitvector n2) (PEqWord n2)) v v = false
-ecFromTo_m_n_equiv
-  : forall m n : Nat, to_list (ecFromTo m n Integer PLiteralInteger) = List.map (Z.add (Z.of_nat m)) (toN_int (n - m))
+ecOr_0_if : forall (n : nat) (x y : bitvector n), ecOr (bitvector n) (PLogicWord n) x y = replicate n bool 0%bool -> x = replicate n bool 0%bool /\ y = replicate n bool 0%bool
+ecNotEq_vec_bv_true : forall (n1 n2 : nat) (v1 v2 : Vec n1 (bitvector n2)), v1 <> v2 -> ecNotEq (Vec n1 (bitvector n2)) (PEqVec n1 (bitvector n2) (PEqWord n2)) v1 v2 = 1%bool
+ecNotEq_vec_bv_false : forall (n1 n2 : nat) (v : Vec n1 (bitvector n2)), ecNotEq (Vec n1 (bitvector n2)) (PEqVec n1 (bitvector n2) (PEqWord n2)) v v = 0%bool
+ecFromTo_m_n_equiv : forall m n : Nat, to_list (ecFromTo m n Integer PLiteralInteger) = List.map (Z.add (Z.of_nat m)) (toN_int (n - m))
 ecFromTo_0_n_equiv : forall n : Nat, to_list (ecFromTo 0%nat n Integer PLiteralInteger) = toN_int n
-ecFromTo_0_n_bv_excl_equiv
-  : forall (s : nat) (n : Nat), to_list (ecFromTo 0%nat n (seq s Bool) (PLiteralSeqBool s)) = toN_excl_bv s (S n)
-ecFoldl_foldl_equiv
-  : forall (A B : Type) (inhB : Inhabited B) (f : A -> B -> A) (n : Nat) (ls : seq n B) (a : A),
-    ecFoldl n A B f a ls = List.fold_left f (to_list ls) a
-ecEq_vec_bv_true
-  : forall (n1 n2 : nat) (v : Vec n1 (bitvector n2)),
-    ecEq (Vec n1 (bitvector n2)) (PEqVec n1 (bitvector n2) (PEqWord n2)) v v = true
-ecEq_vec_bv_false
-  : forall (n1 n2 : nat) (v1 v2 : Vec n1 (bitvector n2)),
-    v1 <> v2 -> ecEq (Vec n1 (bitvector n2)) (PEqVec n1 (bitvector n2) (PEqWord n2)) v1 v2 = false
+ecFromTo_0_n_bv_excl_equiv : forall (s : nat) (n : Nat), to_list (ecFromTo 0%nat n (seq s Bool) (PLiteralSeqBool s)) = toN_excl_bv s (S n)
+ecFoldl_foldl_equiv : forall (A B : Type) (inhB : Inhabited B) (f : A -> B -> A) (n : Nat) (ls : seq n B) (a : A), ecFoldl n A B f a ls = List.fold_left f (to_list ls) a
+ecEq_vec_bv_true : forall (n1 n2 : nat) (v : Vec n1 (bitvector n2)), ecEq (Vec n1 (bitvector n2)) (PEqVec n1 (bitvector n2) (PEqWord n2)) v v = 1%bool
+ecEq_vec_bv_false : forall (n1 n2 : nat) (v1 v2 : Vec n1 (bitvector n2)), v1 <> v2 -> ecEq (Vec n1 (bitvector n2)) (PEqVec n1 (bitvector n2) (PEqWord n2)) v1 v2 = 0%bool
 bvToNat_toZ_equiv : forall (n : Nat) (x : bitvector n), BinInt.Z.of_nat (bvToNat n x) = bvToInt n x
 bvToNat_lt_word : forall (n : Nat) (x : bitvector n), (BinInt.Z.of_nat (bvToNat n x) < 2 ^ BinInt.Z.of_nat n)%Z
-bvToNat_Z_to_nat_equiv
-  : forall (n : Nat) (x : bitvector n) (z : Z), (0 <= z)%Z -> sbvToInt n x = z -> bvToNat n x = BinInt.Z.to_nat z
-bvToInt_shiftR_lt
-  : forall (n : Nat) (v : bitvector n) (s : nat) (b : Z),
-    (bvToInt n v < 2 ^ (BinInt.Z.of_nat s + b))%Z -> (bvToInt n (shiftR n bool false v s) < 2 ^ b)%Z
-bvToInt_shiftR_equiv
-  : forall (n s : nat) (x : t bool n),
-    s >= 0 -> bvToInt n (shiftR n bool false x s) = BinInt.Z.shiftr (bvToInt n x) (BinInt.Z.of_nat s)
-bvToInt_shiftL_1_equiv
-  : forall n s : nat, s < n -> bvToInt n (shiftL n bool false (intToBv n 1) s) = BinInt.Z.shiftl 1 (BinInt.Z.of_nat s)
-bvToInt_sbvToInt_range
-  : forall (n : Nat) (v : bitvector n) (x : Z), (bvToInt n v < 2 ^ (1 + x))%Z -> (- 2 ^ x <= sbvToInt n v < 2 ^ x)%Z
-bvToInt_sbvToInt_equiv
-  : forall (n : nat) (v : bitvector n),
-    n > 0 -> (bvToInt n v < 2 ^ BinInt.Z.of_nat (Nat.pred n))%Z -> sbvToInt n v = bvToInt n v
+bvToNat_Z_to_nat_equiv : forall (n : Nat) (x : bitvector n) (z : Z), (0 <= z)%Z -> sbvToInt n x = z -> bvToNat n x = BinInt.Z.to_nat z
+bvToInt_shiftR_lt : forall (n : Nat) (v : bitvector n) (s : nat) (b : Z), (bvToInt n v < 2 ^ (BinInt.Z.of_nat s + b))%Z -> (bvToInt n (shiftR n bool 0%bool v s) < 2 ^ b)%Z
+bvToInt_shiftR_equiv : forall (n s : nat) (x : t bool n), s >= 0 -> bvToInt n (shiftR n bool 0%bool x s) = BinInt.Z.shiftr (bvToInt n x) (BinInt.Z.of_nat s)
+bvToInt_shiftL_1_equiv : forall n s : nat, s < n -> bvToInt n (shiftL n bool 0%bool (intToBv n 1) s) = BinInt.Z.shiftl 1 (BinInt.Z.of_nat s)
+bvToInt_sbvToInt_range : forall (n : Nat) (v : bitvector n) (x : Z), (bvToInt n v < 2 ^ (1 + x))%Z -> (- 2 ^ x <= sbvToInt n v < 2 ^ x)%Z
+bvToInt_sbvToInt_equiv : forall (n : nat) (v : bitvector n), n > 0 -> (bvToInt n v < 2 ^ BinInt.Z.of_nat (Nat.pred n))%Z -> sbvToInt n v = bvToInt n v
 bvToInt_nonneg : forall (n : Nat) (v : bitvector n), (0 <= bvToInt n v)%Z
 bvToInt_intToBv_id : forall (n : Nat) (v : Z), bvToInt n (intToBv n v) = v
 bvToInt_bvAdd_small_equiv
-  : forall (n : nat) (v1 v2 : bitvector n),
-    (0 <= bvToInt n v1 + sbvToInt n v2 < 2 ^ BinInt.Z.of_nat n)%Z ->
-    bvToInt n (bvAdd n v1 v2) = (bvToInt n v1 + sbvToInt n v2)%Z
+  : forall (n : nat) (v1 v2 : bitvector n), (0 <= bvToInt n v1 + sbvToInt n v2 < 2 ^ BinInt.Z.of_nat n)%Z -> bvToInt n (bvAdd n v1 v2) = (bvToInt n v1 + sbvToInt n v2)%Z
 bvToInt_bound : forall (n : Nat) (v : bitvector n), (0 <= bvToInt n v < 2 ^ BinInt.Z.of_nat n)%Z
+bvToBits_eq_inv : forall (n : nat) (b1 b2 : bitvector n), bvToBITS b1 = bvToBITS b2 -> b1 = b2
 bvToBITS_z_equiv : forall (n : Nat) (z : Z), bvToBITS (intToBv n z) = spec.fromZ z
+bvToBITS_xor_eq : forall (n : Nat) (v1 v2 : bitvector n), bvToBITS (bvXor n v1 v2) = xorB (bvToBITS v1) (bvToBITS v2)
+bvToBITS_ones_eq : forall n : Nat, bvToBITS (replicate n bool 1%bool) = spec.ones n
 bvToBITS_bitsToBv_id : forall (n : nat) (v : spec.BITS n), bvToBITS (bitsToBv v) = v
-bvSShr_all_nonneg
-  : forall (n1 : nat) (v : bitvector (S n1)), (0 <= sbvToInt (S n1) v)%Z -> bvSShr n1 v n1 = replicate (S n1) bool false
-bvSShr_all_neg
-  : forall (n1 : nat) (v : bitvector (S n1)), (sbvToInt (S n1) v < 0)%Z -> bvSShr n1 v n1 = replicate (S n1) bool true
+bvSShr_all_nonneg : forall (n1 : nat) (v : bitvector (S n1)), (0 <= sbvToInt (S n1) v)%Z -> bvSShr n1 v n1 = replicate (S n1) bool 0%bool
+bvSShr_all_neg : forall (n1 : nat) (v : bitvector (S n1)), (sbvToInt (S n1) v < 0)%Z -> bvSShr n1 v n1 = replicate (S n1) bool 1%bool
 bvSShr_Z_shiftr_equiv
   : forall (n : nat) (x1 : bitvector (S n)) (x2 : Z) (y1 : nat) (y2 : Z),
     BinInt.Z.of_nat y1 = y2 -> sbvToInt (S n) x1 = x2 -> sbvToInt (S n) (bvSShr n x1 y1) = BinInt.Z.shiftr x2 y2
 bvOr_bvToInt_equiv : forall (n : Nat) (x y : bitvector n), bvToInt n (bvOr n x y) = BinInt.Z.lor (bvToInt n x) (bvToInt n y)
 bvNat_bvToNat_id : forall (n : Nat) (x : bitvector n), Eq (bitvector n) (bvNat n (bvToNat n x)) x
-bvMul_2_shiftl_equiv : forall (n : nat) (v : bitvector n), bvMul n (intToBv n 2) v = shiftL n bool false v 1
-bvEq_nth_order
-  : forall (n : nat) (v1 v2 : bitvector n),
-    bvEq n v1 v2 = true -> forall (n' : nat) (pf : n' < n), nth_order v1 pf = nth_order v2 pf
-bvEq_false_ne
-  : forall (n : nat) (v1 v2 : bitvector n),
-    bvEq n v1 v2 = false -> exists (n' : nat) (nlt : n' < n), nth_order v1 nlt <> nth_order v2 nlt
+bvMul_2_shiftl_equiv : forall (n : nat) (v : bitvector n), bvMul n (intToBv n 2) v = shiftL n bool 0%bool v 1
+bvEq_nth_order : forall (n : nat) (v1 v2 : bitvector n), bvEq n v1 v2 = 1%bool -> forall (n' : nat) (pf : n' < n), nth_order v1 pf = nth_order v2 pf
+bvEq_false_ne : forall (n : nat) (v1 v2 : bitvector n), bvEq n v1 v2 = 0%bool -> exists (n' : nat) (nlt : n' < n), nth_order v1 nlt <> nth_order v2 nlt
 bits_cons_decomp : forall (n : nat) (v : spec.BITS (S n)), exists (b : bool) (v' : spec.BITS n), v = spec.consB b v'
-bitsToBv_cons_eq
-  : forall (n : nat) (x : spec.BITS n) (h : Bool), VectorDef.cons Bool h n (bitsToBv x) = bitsToBv (spec.consB h x)
+bitsToBv_cons_eq : forall (n : nat) (x : spec.BITS n) (h : Bool), VectorDef.cons Bool h n (bitsToBv x) = bitsToBv (spec.consB h x)
+append_nil_eq : forall (A : Type) (inh : Inhabited A) (n : nat) (v : Vec n A), append 0%nat n A (nil A) v = v
 adcB_0_1_equiv : forall (n : nat) (a : spec.BITS n), adcB 1 (spec.fromZ 0) a = adcB 0 (spec.fromZ 1) a
 JMeq.JMeq_eq : forall (A : Type) (x y : A), JMeq.JMeq x y -> x = y
-Constant CryptolToCoq.SAWCoreVectorsAsCoqVectors.bvToInt
 
 *)
 
@@ -237,6 +162,37 @@ Ltac removeCoerce :=
   | [ |- context[coerce ?t1 ?t2 ?p ?a]] => 
     replace (coerce t1 t2 p a) with a; [idtac | reflexivity]
   end.
+
+Theorem Vec_0_nil : forall (A : Type)(v : Vec O A),
+  v = @Vector.nil A.
+
+  intros.
+  eapply (@case0 _ (fun v => v = Vector.nil A)).
+  reflexivity.
+
+Qed.
+
+Theorem Vec_S_cons : forall (A : Type) n (v : Vec (S n) A),
+  exists x y, v = @Vector.cons A x n y.
+
+  intros.
+  eapply (@VectorDef.caseS' _ _ _ (fun v => exists x y, v = Vector.cons A x n y)).
+  intros.
+  econstructor.
+  econstructor.
+  reflexivity.
+
+Qed.
+
+
+Theorem empty_Vec_eq : forall (A : Type)(v1 v2 : Vec O A),
+  v1 = v2.
+
+  intros.
+  rewrite (@Vec_0_nil _ v1).
+  rewrite (@Vec_0_nil _ v2).
+  reflexivity.
+Qed.
 
 
 Theorem ecScanl_vec_ext : forall t1 t2 (f1 f2 : t1 -> t2 -> t1) n (ls : Vec n t2) x,
@@ -303,12 +259,6 @@ Admitted.
 
 Theorem toList_ecDrop_equiv : forall A (inh : Inhabited A) n m (v : Vec (addNat n m) A),
   to_list (ecDrop n m _ v) = skipn n (to_list v).
-
-Admitted.
-
-Theorem toList_append_equiv : forall A (inh : Inhabited A) n m (v1 : Vec n A)(v2 : Vec m A),
-  to_list (SAWCorePrelude.append _ _ _ v1 v2) = 
-  List.app (to_list v1) (to_list v2).
 
 Admitted.
 
@@ -444,15 +394,6 @@ Theorem ecCat_equiv : forall s1 s2 t (inh : Inhabited t)(a : Vec s1 t) (b : Vec 
 Qed.
 
 
-Theorem to_list_ecCAt_equiv : forall (s1 s2 : nat) t (inh : Inhabited t)(a : Vec s1 t) (b : Vec s2 t),
-  (to_list (ecCat (TCNum s1) (TCNum s2) t a b)) = (List.app (to_list a) (to_list b)).
-
-  intros.
-  rewrite ecCat_equiv.
-  apply toList_append_equiv.
-
-Qed.
-
 Theorem sawAt_nth_equiv : forall (A : Type)(inh : Inhabited A)(n1 : nat)(ls : Vec n1 A)(n2 : nat),
    (n2 < n1)%nat ->
    (sawAt _ _ ls n2) = (nth n2 (to_list ls) (inhabitant inh)).
@@ -477,24 +418,198 @@ Theorem to_list_cons : forall (A : Type)(n : Nat)(ls : Vec n A) x,
 
 Qed.
 
-
+(*
 Theorem toList_reverse_cons_eq : forall (A : Type)(inh : Inhabited A) n (ls : Vec n A) a,
   to_list (SAWCorePrelude.reverse _ _ (Vector.cons _ a _ ls)) =  (to_list (SAWCorePrelude.reverse _ _ ls)) ++ (a :: nil).
+  
+  intros.
+  unfold SAWCorePrelude.reverse.
+  Search gen.
+  specialize (gen_add n 1%nat _ (fun i : Nat => sawAt (S n) A (Vector.cons A a n ls) (subNat (subNat (S n) 1%nat) i))). intros.
+  assert (ssrnat.addn n 1 = S n) by admit.
+  rewrite H0 in H.
+  replace (ssrnat.addn n 1) with (S n).
+  rewrite H.
 
 
-Admitted.
+  induction n; intros; simpl in *.
+  rewrite (Vec_0_nil ls).
+  reflexivity.
+  destruct (Vec_S_cons ls).
+  destruct H.
+  subst.
+  simpl.
+  Search Vec S.
+
+Qed.
+*)
+
+Print rev_ind.
+
+Section NatPlusInd.
+
+  Variable P : nat -> Prop.
+  Hypothesis base : P O.
+  Hypothesis step : forall n, P n -> P (n + 1)%nat.
+
+  Theorem nat_plus_ind : forall n, P n.
+    induction n; intros; simpl in *; trivial.
+    specialize (@step n).
+    replace (S n )%nat with (n + 1)%nat.
+    eauto.
+    lia.
+  Qed.
+
+End NatPlusInd.
+
+Theorem Vec_plus_app : forall (A : Type) n m (v : Vec (n + m)%nat A),
+  exists (v1 : (Vec n A))(v2 : (Vec m A)),
+    v = Vector.append v1 v2.
+
+  induction n; intros; simpl in *.
+  exists (Vector.nil A).
+  exists v.
+  reflexivity.
+
+  destruct (Vec_S_cons v).
+  destruct H.
+  subst.
+  destruct (IHn _ x0). destruct H. subst.
+  exists (Vector.cons A x _ x1).
+  exists x2.
+  simpl.
+  reflexivity.
+
+Qed.
+
+(*
+Require Import Eqdep.
+
+Check eq_dep.
+
+Theorem Vec_rev_append_eq : forall (A : Type) n1 (v1 : Vec n1 A) n2 (v2 : Vec n2 A),
+  eq_dep nat (fun n => Vec n A) _ (Vector.rev (Vector.append v1 v2)) _ (Vector.append (Vector.rev v2) (Vector.rev v1)).
+
+Abort.
+
+Definition Vec_eq_length (A : Type) (n m : nat) (len_eq : n = m) v :=
+  eq_rect _ (fun k => @Vec k A) v _ len_eq.
+*)
+
+
+Fixpoint gen_ls (n : nat)(A : Type)(f : nat -> A) : list A :=
+  match n with
+  | O => nil
+  | S p => cons (f 0%nat) (gen_ls p (fun i => f (S i)))
+  end.
+
+Theorem to_list_gen_sawAt_eq : forall (A : Type)(inh : Inhabited A) n n' (ls : Vec n' A)(f : nat-> nat),
+  (forall i, i < n -> f i < n')%nat -> 
+  to_list (gen n _ (fun i => sawAt n' _ ls (f i) )) = gen_ls n (fun i => nth (f i) (to_list ls) inhabitant). 
+
+  induction n; intros; simpl in *.
+  reflexivity.
+
+  rewrite to_list_cons.
+  rewrite (@IHn _ ls (fun x => (f (S x)))).
+  f_equal.
+  apply sawAt_nth_equiv.
+  eapply H.
+  lia.
+  intros.
+  eapply H.
+  lia.
+
+Qed.
+
+Theorem gen_ls_ext : forall (A : Type) n (f1 f2 : nat -> A),
+  (forall i, (i < n)%nat -> f1 i = f2 i) ->
+  gen_ls n f1 = gen_ls n f2.
+
+  induction n; intros; simpl in *.
+  trivial.
+
+  f_equal.
+  eapply H.
+  lia.
+  eapply IHn.
+  intros.
+  eapply H.
+  lia.
+
+Qed.
+
+
+Theorem gen_ls_reverse_equiv : forall (A : Type)(inh : Inhabited A) n (ls : list A) , 
+  length ls = n ->
+  gen_ls n (fun i : nat => nth ((n - 1) - i)%nat ls inhabitant) = rev ls.
+
+  induction n; intuition; simpl in *.
+  destruct ls; simpl in *; trivial; try discriminate.
+
+  destruct ls using rev_ind.
+  simpl in *. discriminate.
+  rewrite app_length in H.
+  assert (n = Datatypes.length ls).
+  simpl in *. lia.
+  subst.
+  rewrite rev_app_distr.
+  simpl.
+  f_equal.
+  rewrite app_nth2.
+  simpl in *.
+  repeat rewrite Nat.sub_0_r.
+  rewrite minus_diag. trivial.
+  lia.
+
+  specialize (IHn ls).
+  rewrite <- IHn; trivial.
+  eapply gen_ls_ext.
+  intros.
+  repeat rewrite Nat.sub_0_r.
+  replace (Datatypes.length ls - 1 - i)%nat with (Datatypes.length ls - (S i))%nat.
+  rewrite app_nth1.
+  trivial.
+  lia.
+  lia.
+ 
+Qed.
+
+Theorem gen_ls_reverse_subNat_equiv : forall (A : Type)(inh : Inhabited A) n (ls : list A) , 
+  length ls = n ->
+  gen_ls n (fun i : nat => nth (subNat (subNat n 1%nat) i) ls inhabitant) = rev ls.
+
+  intros.
+  erewrite gen_ls_ext.
+  apply gen_ls_reverse_equiv; eauto.
+  intros.  
+  repeat rewrite subNat_sub.
+  reflexivity.
+Qed.
+
+
+Theorem to_list_length : forall (A : Type) n (ls : Vec n A),
+  List.length (to_list ls) = n.
+
+  induction ls; intros.
+  trivial.
+  rewrite to_list_cons.
+  simpl.
+  f_equal; eauto.
+
+Qed.
 
 Theorem toList_reverse_equiv : forall (A : Type)(inh : Inhabited A) n (ls : Vec n A),
   to_list (SAWCorePrelude.reverse _ _ ls) = rev (to_list ls).
 
-
-  induction ls; intros.
-  simpl in *.
-  trivial.
-  rewrite toList_cons.
-  simpl.
-  rewrite <- IHls.
-  apply toList_reverse_cons_eq.
+  intros.
+  unfold reverse.
+  rewrite to_list_gen_sawAt_eq.
+  apply gen_ls_reverse_subNat_equiv.
+  apply to_list_length.
+  intros.
+  repeat rewrite subNat_sub.
+  lia.
 
 Qed.
 
@@ -566,27 +681,6 @@ Theorem zip_cons_equiv : forall A B (inha : Inhabited A)(inhb : Inhabited B) n (
 
 Qed.
 
-Theorem Vec_0_nil : forall (A : Type)(v : Vec O A),
-  v = @Vector.nil A.
-
-  intros.
-  eapply (@case0 _ (fun v => v = Vector.nil A)).
-  reflexivity.
-
-Qed.
-
-Theorem Vec_S_cons : forall (A : Type) n (v : Vec (S n) A),
-  exists x y, v = @Vector.cons A x n y.
-
-  intros.
-  eapply (@VectorDef.caseS' _ _ _ (fun v => exists x y, v = Vector.cons A x n y)).
-  intros.
-  econstructor.
-  econstructor.
-  reflexivity.
-
-Qed.
-
 Theorem toList_zip_equiv : forall (A B : Type)(inha : Inhabited A)(inhb: Inhabited B) n (lsa: Vec n A) (lsb : Vec n B),
   to_list (zip (TCNum n) lsa lsb) = List.combine (to_list lsa) (to_list lsb).
 
@@ -618,10 +712,34 @@ Theorem fold_left_ext : forall (A B : Type)(f1 f2 : A -> B -> A) ls a,
   intuition idtac.  
 Qed.
 
+Theorem drop_cons_eq : forall (A : Type)(inh : Inhabited A) n1 n2 ls a,
+  drop A (S n1) n2 (Vector.cons _ a _ ls) = drop A n1 n2 ls.
+
+  intros.
+  reflexivity.
+
+Qed.
+
 Theorem toList_drop_equiv : forall A (inh : Inhabited A) n1 n2 ls,
   to_list (drop A n1 n2 ls) = skipn n1 (to_list ls).
 
-Admitted.
+  induction n1; intros; simpl in *.
+  unfold drop.
+  erewrite gen_domain_eq.
+  rewrite gen_sawAt.
+  reflexivity.
+  intros.
+  simpl.
+  reflexivity.
+
+  destruct (Vec_S_cons ls). destruct H.
+  subst.
+  rewrite drop_cons_eq.
+  rewrite IHn1.
+  rewrite to_list_cons.
+  reflexivity.
+
+Qed.
 
 Theorem nth_order_S_cons : forall (A : Type) a n (v : Vec n A) n' (pf : (S n' < S n)%nat)(pf' : (n' < n)%nat),
   nth_order (Vector.cons _ a _ v) pf = nth_order v pf'.
@@ -637,11 +755,21 @@ Theorem ssr_addn_even : forall n1 n2,
   even n1 = true ->
   even n2 = true ->
   even (ssrnat.addn n1 n2) = true.
-Admitted.
+
+  intros.
+  rewrite <- ssrnat.plusE.
+  rewrite Nat.even_add_even; trivial.
+  apply Nat.even_spec; trivial.
+
+Qed.
+
 
 Theorem ssr_double_even : forall n,
   even (ssrnat.double n) = true.
-Admitted.
+
+  induction n; intros; simpl in *; trivial.
+
+Qed.
 
 Theorem nth_order_0_cons : forall (A : Type) a n (v : Vec n A) (pf : (0 < S n)%nat),
   nth_order (Vector.cons _ a _ v) pf = a.
@@ -897,6 +1025,7 @@ Theorem bvAnd_drop_equiv: forall n1 n2 v1 v2,
 
 Qed.
 
+
 Theorem intToBv_1_append_eq : forall n1 n2,
   (n1 > 0)%nat ->
   append (intToBv n2 0) (intToBv n1 1) = intToBv (addNat n2 n1) 1.
@@ -906,15 +1035,6 @@ Theorem intToBv_1_append_eq' : forall n1 n2,
   (n1 > 0)%nat ->
   Vector.append (intToBv n2 0) (intToBv n1 1) = intToBv (n2 + n1)%nat 1.
 Admitted.
-
-Theorem empty_Vec_eq : forall (A : Type)(v1 v2 : Vec O A),
-  v1 = v2.
-
-  intros.
-  rewrite (@Vec_0_nil _ v1).
-  rewrite (@Vec_0_nil _ v2).
-  reflexivity.
-Qed.
 
 Theorem bvAnd_lsb_drop_equiv: forall n1 n2 v,
   (bvAnd (@drop _ _ n2 n1 v) (intToBv _ 1)) = 
@@ -933,6 +1053,7 @@ Theorem bvAnd_lsb_drop_equiv: forall n1 n2 v,
   trivial.
 
 Qed.
+
 
 
 Theorem bvAnd_0 : forall n (v : Vec n _),
@@ -1039,9 +1160,18 @@ Theorem bvToNat_toZ_equiv : forall n x,
   (BinInt.Z.of_nat (bvToNat n x)) = bvToInt n x.
 Admitted.
 
+
 Theorem sbvToInt_bvToInt_id : forall n x,
+  (n > 0)%nat -> 
   intToBv n (sbvToInt n x) = x.
+
+  intros.
+  unfold intToBv, sbvToInt.
+  destruct n.
+  lia.
+  Print spec.toZ.
 Admitted.
+
 
 Theorem ecEq_bv_true : forall n v,  
   ecEq (bitvector n) (PEqWord n) v v = true.
@@ -1319,12 +1449,6 @@ Theorem bvToInt_intToBv_id : forall n v,
 
 Admitted.
 
-Theorem sbvToInt_intToBv_id : forall n v,
-  (-Z.pow 2 (Z.of_nat (pred n)) <= v < Z.pow 2 (Z.of_nat (pred n)))%Z ->
-  sbvToInt n (intToBv n v) = v.
-
-Admitted.
-
 Theorem sbvToInt_bvURem_equiv : forall n v1 v2,
   (n > 0)%nat ->
   (0 < bvToInt _ v2)%Z ->
@@ -1354,20 +1478,40 @@ Theorem bvMul_2_shiftl_equiv : forall n v,
   bvMul n (intToBv _ 2) v = shiftL _ _ false v 1.
 Admitted.
 
+Theorem shiftL1_shiftL : forall (A : Type) n (b : A) v n1,
+  (shiftL1 n _ b (shiftL n _ b v n1)) = shiftL n _ b v (S n1).
+
+  induction n1; intros; simpl in *.
+  reflexivity.
+  reflexivity.
+
+Qed.
+
+Theorem shiftL_shiftL1 : forall (A : Type) n (b : A) v n1,
+  (shiftL n _ b (shiftL1 n _ b v) n1) = shiftL n _ b v (S n1).
+
+  induction n1; intros; simpl in *.
+  reflexivity.
+  rewrite IHn1.
+  reflexivity.
+
+Qed.
+
 Theorem shiftL_shiftL : forall (A : Type) n (b : A) v n1 n2,
   (shiftL n _ b (shiftL n _ b v n1) n2) = shiftL n _ b v (n1 + n2).
-Admitted.
+
+  induction n1; intros; simpl in *; trivial.
+  rewrite shiftL_shiftL1.
+  rewrite IHn1.
+  rewrite shiftL1_shiftL.
+  f_equal.
+  lia.
+
+Qed.
 
 Theorem bvToInt_shiftL_1_equiv : forall n s,
   (s < n)%nat ->
   bvToInt n (shiftL _ _ false (intToBv _ 1) s) = 
-  Z.shiftl 1 (Z.of_nat s).
-Admitted.
-
-Theorem sbvToInt_shiftL_1_equiv : forall n s,
-  (n > 0)%nat ->
-  (s < pred n)%nat ->
-  sbvToInt n (shiftL _ _ false (intToBv _ 1) s) = 
   Z.shiftl 1 (Z.of_nat s).
 Admitted.
 
@@ -1737,6 +1881,16 @@ Theorem intToBv_0_S : forall n,
 
  Admitted.
 
+(*
+Theorem intToBv_add_equiv_64 : forall x y,
+  intToBv 64%nat (x + y) = bvAdd 64%nat (intToBv 64%nat x) (intToBv 64%nat y).
+
+  intros.
+  lia.
+
+Qed.
+*)
+
 Theorem intToBv_add_equiv : forall n x y,
   intToBv n (x + y) = bvAdd n (intToBv n x) (intToBv n y).
 
@@ -1779,16 +1933,8 @@ Theorem sbvToInt_0_replicate: forall n b2,
     b2 = replicate _ _ false.
 Admitted.
 
-Theorem shiftR_false_0 : forall n1 n2, 
-    (shiftR n1 bool false (replicate n1 bool false) n2) = (replicate n1 bool false).
-Admitted.
-
 Theorem bvNeg_replicate_0 : forall n,
     bvNeg _ (replicate n bool false) = replicate n bool false.
-Admitted.
-
-Theorem sbvToInt_replicate_0 : forall n,
-  sbvToInt _ (replicate n bool false) = 0.
 Admitted.
 
 Theorem shiftR_small_nonneg : forall n1 n2 v,
@@ -1796,10 +1942,7 @@ Theorem shiftR_small_nonneg : forall n1 n2 v,
   (shiftR n1 bool false v n2) = replicate n1 bool false.
 Admitted.
 
-Theorem shiftR_all_nonneg : forall n1 v,
-  (0 <= sbvToInt _ v)%Z ->
-  (shiftR n1 bool false v (pred n1)) = replicate n1 bool false.
-Admitted.
+
 
 Theorem bvSShr_all_nonneg : forall n1 v,
   (0 <= sbvToInt _ v)%Z ->
@@ -2002,6 +2145,7 @@ Theorem foldl_dep_tuple_cat : forall n1 (x : Vector.t bool n1) n2 (v : tuple.tup
 Admitted.
 *)
 
+(*
 Theorem foldl_dep_tuple_cons : forall n (x : Vector.t bool n) b,
   foldl_dep bool (fun n0 : Nat => tuple.tuple_of (S n0) bool) n
   (fun (n0 : Nat) (bs : tuple.tuple_of (S n0) bool) (b0 : bool) =>
@@ -2011,7 +2155,13 @@ Theorem foldl_dep_tuple_cons : forall n (x : Vector.t bool n) b,
   foldl_dep bool (fun n0 : Nat => tuple.tuple_of n0 bool) n
   (fun (n0 : Nat) (bs : tuple.tuple_of n0 bool) (b0 : bool) =>
    tuple.cons_tuple b0 bs) (tuple.nil_tuple bool) x).
-Admitted.
+
+  induction x; intros; simpl in *.
+  reflexivity.
+
+  
+
+Qed.
 
 Theorem bvToBITS_cons_eq : forall n (x : Vector.t bool n) b,
   bvToBITS (Vector.cons b x) =
@@ -2029,12 +2179,16 @@ Theorem bvToBITS_cons_eq : forall n (x : Vector.t bool n) b,
 
 Qed.
 
+*)
+
 Theorem xorB_cons : forall n (v1 v2 : spec.BITS n) b1 b2,
   xorB (spec.consB b1 v1) (spec.consB b2 v2) = spec.consB (xorb b1 b2) (xorB v1 v2).
 
   intros.
   apply liftBinOpCons.
 Qed.
+
+(*
 
 Theorem bvToBITS_xor_eq : forall n v1 v2, 
   bvToBITS (bvXor n v1 v2) = xorB (bvToBITS v1) (bvToBITS v2).
@@ -2057,6 +2211,20 @@ Theorem bvToBITS_xor_eq : forall n v1 v2,
 
 Qed.
 
+*)
+
+Theorem bvToBITS_xor_eq : forall n v1 v2, 
+  bvToBITS (bvXor n v1 v2) = xorB (bvToBITS v1) (bvToBITS v2).
+
+Admitted.
+
+Theorem bvToBITS_ones_eq : forall n,
+  bvToBITS (replicate n bool true) = spec.ones n.
+
+Admitted.
+
+(*
+
 Theorem bvToBITS_ones_eq : forall n,
   bvToBITS (replicate n bool true) = spec.ones n.
 
@@ -2069,6 +2237,8 @@ Theorem bvToBITS_ones_eq : forall n,
   apply bvToBITS_cons_eq.
 
 Qed.
+
+*)
 
 
 Theorem twos_complement_equiv : forall n v,
@@ -2096,18 +2266,8 @@ Theorem twos_complement_equiv : forall n v,
 Qed.
 
 
-Theorem intToBv_0_eq_replicate : forall n,
-    intToBv n 0 = replicate n bool false.
-Admitted.
-
 Theorem sawAt_nth_order_equiv : forall (A : Type)(inh : Inhabited A)(n1 n2 : nat)(v : Vec n1 A)(ltpf : (n2 < n1)%nat),
   @sawAt n1 A inh v n2 = nth_order v ltpf.
-Admitted.
-
-Theorem sbvToInt_nz_nth : forall n (v : Vec n _) n' (nlt : (n' < n)%nat),
-  nth_order v nlt = true ->
-  sbvToInt _ v <> 0%Z.
-
 Admitted.
 
 Theorem shiftR_shiftR_eq : forall (A : Type)(n1 n2 len : nat)(v : Vec len A) a,
@@ -2129,11 +2289,6 @@ Admitted.
 Theorem nth_order_shiftR_all_eq : forall (A : Type)(n2 len : nat)(v : Vec len A) (nlt : (n2 < len)%nat)(zlt : (0 < len)%nat) a,
   nth_order (shiftR _ _ a v n2) nlt = nth_order v zlt.
 
-Admitted.
-
-Theorem sbvToInt_neg_sign_bit_set : forall n  b2 (ltpf : (0 < n)%nat),
-    (sbvToInt n b2 < 0)%Z ->
-    nth_order b2 ltpf = true.
 Admitted.
 
 Theorem sbvToInt_neg_bits_set : forall n wsize b2 n' (ltpf : (n' < n)%nat),
@@ -2241,6 +2396,7 @@ Theorem bitsToBv_eq_inv : forall n (b1 b2 : spec.BITS n),
 
 Qed.
 
+(*
 Theorem bvToBits_eq_inv : forall n (b1 b2 : bitvector n),
   bvToBITS b1 = bvToBITS b2 ->
   b1 = b2.
@@ -2263,6 +2419,12 @@ Theorem bvToBits_eq_inv : forall n (b1 b2 : bitvector n),
   eauto.
 
 Qed.
+*)
+Theorem bvToBits_eq_inv : forall n (b1 b2 : bitvector n),
+  bvToBITS b1 = bvToBITS b2 ->
+  b1 = b2.
+
+Admitted.
 
 Theorem addb_same_l : forall n (x y1 y2 : spec.BITS n),
   y1 = y2 ->
@@ -2406,12 +2568,6 @@ Theorem nth_order_eq_impl_eq : forall (A : Type) n (v1 v2 : Vec n A),
   eapply H.
 Qed.
 
-Theorem shiftR_all_neg : forall n1 v,
-  (sbvToInt _ v < 0)%Z ->
-  (shiftR n1 bool false v (pred n1)) = intToBv _ 1.
-
-Admitted.
-
 
 Theorem bvSShr_all_neg : forall n1 v,
   (sbvToInt _ v < 0)%Z ->
@@ -2419,33 +2575,2008 @@ Theorem bvSShr_all_neg : forall n1 v,
 
 Admitted.
 
-(*
-Theorem bvAnd_shiftR_small_neg : forall n1 n2 v,
-  (-2^(Z.of_nat n2) <= sbvToInt _ v < 0)%Z ->
-  (bvAnd (shiftR n1 bool false v n2) (intToBv _ 1)) = intToBv _ 1.
+Theorem toList_append_equiv : forall A (inh : Inhabited A) n m (v1 : Vec n A)(v2 : Vec m A),
+  to_list (SAWCorePrelude.append v1 v2) = 
+  List.app (to_list v1) (to_list v2).
+
+  induction n; intros; simpl in *.
+  
+  rewrite (Vec_0_nil v1).
+  simpl.
+  rewrite append_nil_eq.
+  reflexivity.
+
+  destruct (Vec_S_cons v1). destruct H. subst.
+  rewrite append_cons.
+  repeat rewrite to_list_cons.
+  rewrite IHn.
+  simpl.
+  reflexivity.
+
+Qed.
+
+
+Theorem to_list_ecCAt_equiv : forall (s1 s2 : nat) t (inh : Inhabited t)(a : Vec s1 t) (b : Vec s2 t),
+  (to_list (ecCat (TCNum s1) (TCNum s2) t a b)) = (List.app (to_list a) (to_list b)).
 
   intros.
+  rewrite ecCat_equiv.
+  apply toList_append_equiv.
 
-  destruct (eq_nat_dec n1 0%nat).
-  subst.
+Qed.
+
+Theorem shiftout_cons : forall (A : Type)(a : A) n (v : Vec (S n) A),
+  shiftout (Vector.cons a v) = Vector.cons a (shiftout v).
+
+  intros.
+  reflexivity.
+
+Qed.
+
+Theorem shiftR1_false_0 : forall n1, 
+    (shiftR1 n1 bool false (replicate n1 bool false)) = (replicate n1 bool false).
+
+  induction n1; intros; simpl in *.
   apply vec_0_eq.
 
-  assert (exists n1', n1 = n1'  + 1)%nat.
-  destruct n1.
-  lia.
-  exists n1.
-  lia.
-
-  destruct H0.
-  subst.
-
-  rewrite <- intToBv_1_append_eq'.
-  rewrite <- (vec_split_append_eq _ _ (shiftR  (x + 1)%nat bool false v n2)).
-  rewrite bvAnd_append'.
+  repeat rewrite replicate_S_cons.
+  unfold shiftR1.
+  rewrite shiftout_cons.
   f_equal.
-  apply bvAnd_0.
+  eapply IHn1.
+
+Qed.
+
+Theorem shiftR_false_0 : forall n2 n1, 
+    (shiftR n1 bool false (replicate n1 bool false) n2) = (replicate n1 bool false).
+
+  induction n2; intros; simpl in *; trivial.
+  rewrite IHn2.
+  eapply shiftR1_false_0.
+
+Qed.
+
+Theorem eq_if_to_list_eq : forall (A : Type) n (v1 v2 : Vector.t A n),
+  to_list v1 = to_list v2 ->
+  v1 = v2.
+
+  induction n; intros; simpl in *.
+  eapply vec_0_eq.
+  destruct (Vec_S_cons v1). destruct H0. subst.
+  destruct (Vec_S_cons v2). destruct H0. subst.
+  repeat rewrite to_list_cons in H.
+  inversion H; clear H; subst.
+  f_equal.
+  eapply IHn.
+  eauto.
+
+Qed.
+
+Theorem toNegZ_nonneg : 
+  forall n (b : spec.BITS n),
+  0 <= spec.toNegZ b.
+
+  induction n; intros; simpl in *.
+  destruct b.
+  destruct tval.
+  unfold spec.toNegZ.
+  simpl.
+  lia.
+  inversion i.
+
+  destruct (bits_cons_decomp b). destruct H. subst.
+  unfold spec.toNegZ in *.
+  simpl in *.
+  destruct x.
+  specialize (IHn x0).
+  lia.
+  specialize (IHn x0).
+  lia.
+
+Qed.
+
+(*
+
+Theorem msb_hd_eq : forall n (v : bitvector (S n)),
+  spec.msb (bvToBITS v) = Vector.hd v.
+
+  intros; simpl in *.
+  destruct (Vec_S_cons v). destruct H. subst.
+  simpl.
+  Print spec.msb.
+  unfold bvToBITS.
+  Search foldl_dep Vector.cons.
+  simpl.
+
+Qed.
+
+Theorem sbvToInt_nonneg_sign_bit_clear:
+  forall [n : nat] (b2 : bitvector n) (ltpf : (0 < n)%nat), 0 <= sbvToInt n b2 -> nth_order b2 ltpf = 0%bool.
+
+  intros.
+  unfold sbvToInt in *.
+  destruct b2; simpl in *.
+  lia.
+  unfold spec.toZ in *.
+  case_eq (spec.splitmsb (bvToBITS (VectorDef.cons h b2))); intros.
+  rewrite H0 in H.
+  destruct b.
+  specialize (toNegZ_nonneg b0); intros.
+  lia.
+
+  Search spec.splitmsb.
+  rewrite splitmsb_msb in H0.
+  Search spec.splitmsb.
+  Print spec.toNegZ.
+  admit.
+  Search spec.toNegZ.
+  Check spec.toNegZ.
+
+  induction b2; intros.
+  lia.
+
+  simpl in *.
+  unfold nth_order.
+  simpl.
+  unfold spec.toZ in *.
+  unfold bvToBITS in *.
+  simpl.
+
+Qed.
+*)
+
+Theorem replicate_repeat_eq : forall n (A  : Type)(v : A),
+  repeat v n = to_list (replicate n A v).
+
+  induction n; intros; simpl in *.
+  rewrite (Vec_0_nil (replicate 0%nat A v)).
+  reflexivity.
+  rewrite replicate_S_cons.
+  rewrite to_list_cons.
+  f_equal.
+  eauto.
+
+Qed.
+
+Definition shiftout_ls (A : Type)(ls : list A):=
+  (firstn (pred (length ls)) ls).
+
+Definition shiftR1_ls (A : Type)(a : A)(ls : list A) :=
+  shiftout_ls (cons a ls).
+
+Theorem shiftR1_ls_equiv : forall (A : Type) n  (v : Vector.t A n) a,
+  to_list (shiftR1 n A a v) = shiftR1_ls a (to_list v).
+
+  induction v; intros; simpl in *.
+  reflexivity.
+
+  unfold shiftR1 in *.
+  rewrite shiftout_cons.
+  rewrite to_list_cons.
+  rewrite IHv.
+  reflexivity.
+
+Qed.
+
+Definition shiftR_ls (A : Type) (x : A) (v :list A) (i : nat) := 
+  ssrnat.iter i (shiftR1_ls x) v.
+
+Theorem shiftR_ls_equiv : forall (A : Type) n2  n (v : Vector.t A n) a,
+  to_list (shiftR n A a v n2) = shiftR_ls a (to_list v) n2.
+
+  induction n2; intros; simpl in *; trivial.
+
+  rewrite shiftR1_ls_equiv.
+  rewrite IHn2.
+  reflexivity.
+
+Qed.
+
+Theorem shiftR1_ls_length : forall (A: Type) a (ls : list A),
+  length (shiftR1_ls a ls) = length ls.
+
+  intros.
+  unfold shiftR1_ls, shiftout_ls.
+  simpl.
+  rewrite firstn_length.
+  simpl.
+  lia.
+
+Qed.
+
+Theorem shiftR_ls_length : forall (A: Type) a n (ls : list A),
+  length (shiftR_ls a ls n) = length ls.
+
+  induction n; intros; simpl in *; trivial.
+  rewrite shiftR1_ls_length.
+  eapply IHn.
+
+Qed.
+
+Theorem firstn_app_1 : forall (A : Type)(ls1 ls2 : list A) n,
+  (n <= length ls1)%nat -> 
+  firstn n (ls1 ++ ls2) = firstn n ls1.
+
+  induction ls1; intros; destruct n; simpl in *; trivial.
+  lia.
+  f_equal.
+  eapply IHls1.
+  lia.
+
+Qed.
+
+Theorem shiftR1_ls_firstn : forall (A : Type) n (ls : list A) a,
+  (n <= length ls)%nat ->
+  firstn n (shiftR1_ls a ls) = shiftR1_ls a (firstn n ls).
+
+  intros. 
+  unfold shiftR1_ls, shiftout_ls.
+  simpl.
+  rewrite firstn_length.
+  rewrite Nat.min_l; trivial.
+  rewrite firstn_firstn.
+  rewrite Nat.min_l; trivial.
+  destruct n.
+  simpl in *; trivial.
+  repeat rewrite firstn_cons.
+  f_equal.
+  rewrite firstn_firstn.
+  rewrite Nat.min_l; trivial; lia.
+
+Qed.
 
 
+Theorem shiftR_ls_firstn : forall (A : Type) n2 n (ls : list A) a,
+  (n <= length ls)%nat ->
+  firstn n (shiftR_ls a ls n2) = shiftR_ls a (firstn n ls) n2.
+
+  induction n2; intros; simpl in *; trivial.
+  rewrite shiftR1_ls_firstn.
+  rewrite IHn2.
+  reflexivity.
+  trivial.
+  rewrite shiftR_ls_length.
+  trivial.
+
+Qed.
+
+
+Theorem shiftR_ls_eq_repeat : forall (A : Type) n (ls : list A) a,
+  (n <= length ls)%nat -> 
+  shiftR_ls a ls n = (repeat a n) ++ (firstn (length ls - n)%nat ls).
+
+  induction n; intros; simpl in *.
+  rewrite Nat.sub_0_r.
+  rewrite firstn_all. reflexivity.
+  unfold shiftR1_ls, shiftout_ls.
+  simpl.
+  rewrite shiftR_ls_length.
+
+  destruct ls using rev_ind.
+  simpl in *. lia.
+  rewrite app_length.
+  simpl.
+  rewrite plus_comm.
+  simpl.
+  f_equal.
+  rewrite firstn_app_1; try lia.
+  rewrite <- IHn.
+  rewrite shiftR_ls_firstn.
+  rewrite firstn_app_1; try lia.
+  rewrite firstn_all.
+  reflexivity.
+  rewrite app_length.
+  lia.
+  rewrite app_length in H.
+  simpl in *. lia.
+Qed.
+
+Definition joinlsb_ls(pair : (list bool) * bool) := (snd pair) :: (fst pair).
+
+(*
+This is not right---list is reversed
+Definition bvToBITS_ls(n : nat)(v : Vec n bool) := to_list v.
+*)
+
+Theorem foldl_dep_conv_const_equiv : forall (A : Type) n (v : Vec n A)
+  (B1 : nat -> Type)(B2 : Type)
+  (conv : forall n, B1 n -> B2) b1
+  (f1 : forall (n : nat), B1 n -> A -> B1 (S n))(f2 : B2 -> A -> B2),
+  (forall n b a, conv _ (f1 n b a) = f2 (conv _ b) a) ->
+  conv _ (foldl_dep A B1 n f1 b1 v) = foldl_dep A (fun _ => B2) n (fun _ => f2) (conv _ b1) v.
+
+  induction v; intros; simpl in *.
+  trivial.
+  specialize (IHv (fun n => B1 (S n)) B2).
+  specialize (IHv (fun n => conv (S n))).
+  specialize (IHv (f1 _ b1 h)).
+  
+  specialize (IHv (fun n0 : nat => f1 (S n0)) f2).
+  simpl in *.
+  unfold Nat in *.
+  rewrite IHv.
+  rewrite H.
+  reflexivity.
+
+  intros.
+  eapply H.
+
+Qed.
+
+Theorem fold_dep_ls_equiv : forall (A : Type) n (v : Vec n A)
+  (B : Type)(f : B -> A -> B) b,
+  foldl_dep A (fun _ => B) n (fun _ => f) b v = fold_left f (to_list v) b.
+
+  induction v; intros.
+  simpl in *.
+  trivial.
+  rewrite to_list_cons.
+  simpl.
+  rewrite IHv.
+  reflexivity.
+
+Qed.
+
+
+Definition bvToBITS_ls_0 n (bs : Vec n bool) :=
+  fold_left (fun (bs : list bool) (b : bool) => b ::bs)(to_list  bs) nil.
+
+
+Theorem bvToBITS_ls_0_equiv : forall n (bs : Vec n bool),
+  tuple.tval (bvToBITS bs) = bvToBITS_ls_0 bs.
+
+  intros.
+  unfold bvToBITS, bvToBITS_ls_0.
+  rewrite <- fold_dep_ls_equiv.
+  specialize (foldl_dep_conv_const_equiv bs spec.BITS (fun n b => tuple.tval b)); intros.
+  simpl in *.
+  eapply H.
+  intros.
+  simpl.
+  reflexivity.
+Qed.
+
+Definition bvToBITS_ls n (bs : Vec n bool) := rev (to_list bs).
+
+Theorem bvToBITS_ls_0_equiv' : forall n (bs : Vec n bool),
+  bvToBITS_ls_0 bs = bvToBITS_ls bs.
+
+  intros. 
+  unfold bvToBITS_ls_0, bvToBITS_ls.
+  generalize (to_list bs) as ls.
+  induction ls using rev_ind; intros; simpl in *.
+  reflexivity.
+
+  rewrite rev_app_distr.
+  rewrite fold_left_app.
+  simpl.
+  f_equal.
+  eauto.
+
+Qed.
+
+Theorem bvToBITS_ls_equiv : forall n (bs : Vec n bool),
+  tuple.tval (bvToBITS bs) = bvToBITS_ls bs.
+
+  intros.
+  rewrite bvToBITS_ls_0_equiv.
+  rewrite bvToBITS_ls_0_equiv'.
+  reflexivity.
+Qed.
+
+Definition splitmsb_ls(ls : list bool):=
+  match (seq.rev ls) with
+  | nil => (false, nil)
+  | b :: ls' => (b, seq.rev ls')
+  end.
+
+Definition toPosZ_ls bs :=
+  seq.foldr (fun (b : bool) (z : Z) => if b then Z.succ (Z.double z) else Z.double z) 0 bs.
+
+Definition toNegZ_ls bs :=
+  seq.foldr (fun (b : bool) (z : Z) => if b then Z.double z else Z.succ (Z.double z)) 0 bs.
+
+Definition toZ_ls bs :=
+  let (b, bs') := splitmsb_ls bs in if b then - Z.succ (toNegZ_ls bs') else toPosZ_ls bs'.
+
+
+Definition sbvToInt_ls n (v : Vec n bool) :=
+  (match n as n0 return (bitvector n0 -> Z) with
+    | 0%nat => fun _ : bitvector 0 => 0
+    | S n0 => fun b0 : bitvector (S n0) => toZ_ls (bvToBITS_ls b0)
+  end) v.
+
+
+(*
+Theorem bvToBITS_ls_eq : forall n (v : Vec n bool) n2 (bs : spec.BITS n2),
+  tuple.tval
+  (foldl_dep bool (fun n0 => spec.BITS (n0 + n2)) n (fun (n0 : Nat) (bs : spec.BITS (n0 + n2)) (b : bool) => spec.joinlsb (bs, b)) 
+     bs v) = seq.rev (to_list v) ++ (tuple.tval bs).
+
+
+Theorem bvToBITS_ls_eq_h : forall n (v : Vec n bool) n2 (bs : spec.BITS n2),
+  tuple.tval
+  (foldl_dep bool (fun n0 => spec.BITS (n0 + n2)) n (fun (n0 : Nat) (bs : spec.BITS (n0 + n2)) (b : bool) => spec.joinlsb (bs, b)) 
+     bs v) = seq.rev (to_list v) ++ (tuple.tval bs).
+
+  induction v; intros; simpl in *.
+  reflexivity.
+  rewrite to_list_cons.
+  
+
+  Check ((spec.joinlsb (tuple.nil_tuple bool, h))).
+  Check (foldl_dep bool (fun n0 : Nat => spec.BITS (S n0)) n
+     (fun (n0 : Nat) (bs : spec.BITS (S n0)) (b : bool) => spec.joinlsb (bs, b)) (spec.joinlsb (tuple.nil_tuple bool, h)) v).
+  Check (foldl_dep bool (fun n0 : Nat => spec.BITS (S n0)) n
+     (fun (n0 : Nat) (bs : spec.BITS (S n0)) (b : bool) => spec.joinlsb (bs, b)) ).
+  Check (foldl_dep bool (fun n0 : Nat => spec.BITS (S n0))).
+
+Qed.
+*)
+
+(*
+
+Theorem foldl_dep_ls_equiv : forall (A : Type) n (v : Vec n A) (B1 : Nat->Type) b1 (f1 : forall (n : Nat), B1 n -> A -> B1 (S n))
+    (B2 : Type)(convB : forall (n : Nat), B1 n -> B2)(f2 : B2 -> A -> B2), 
+    (forall n (b : B1 n) a, convB _ (f1 _ b a) = f2 (convB _ b) a) ->
+    convB _ (foldl_dep A B1 n f1 b1 v) = fold_left f2 (to_list v) (convB _ b1).
+
+  induction v; intros. simpl in *.
+  reflexivity.
+
+  rewrite to_list_cons.
+  simpl.
+  rewrite <- H.
+  rewrite <- IHv.
+
+Qed.
+
+
+Theorem foldl_dep_BITS_foldl_eq : forall n v (f1 : forall n, spec.BITS n -> bool -> spec.BITS (S n)) f2 acc,
+  (forall n (bs : spec.BITS n) (b : bool), tuple.tval (f1 n bs b) = f2 (tuple.tval bs) b) ->
+  tuple.tval (foldl_dep bool spec.BITS n f1 acc v) =
+  fold_left f2 (to_list v)  (tuple.tval acc).
+
+  induction v; intros; simpl in *.
+  reflexivity.
+
+  
+
+  unfold to_list.
+  unfold fold_left.
+  simpl.
+  Search to_list VectorDef.nil.
+  reflexivity.
+  
+
+Qed.
+  
+
+Theorem bvToBITS_ls_eq : forall n (v : Vec n bool),
+ tuple.tval (bvToBITS v) = seq.rev (to_list v).
+
+  intros.
+  unfold bvToBITS.
+  Print foldl_dep.
+
+
+
+  induction v; intros; simpl in *.
+  reflexivity.
+
+  Search seq.rev.
+
+Qed.
+
+Theorem bvToBITS_cons_eq : forall n (v : Vec n bool) h,
+ tuple.tval (bvToBITS (VectorDef.cons h v)) = tuple.tval (bvToBITS v) ++ [h].
+
+  induction v; intros; simpl in *; trivial.
+
+  rewrite IHv.
+
+  unfold bvToBITS.
+
+Qed.
+
+Theorem bvToBITS_ls_equiv : forall n (v : Vec n bool),
+  bvToBITS_ls v = (tuple.tval (bvToBITS v)).
+
+  intros.
+  induction v; intros; simpl in *.
+  reflexivity.
+
+  unfold bvToBITS_ls in *.
+  rewrite to_list_cons.
+  rewrite IHv.
+  rewrite bvToBITS_cons_eq.
+  simpl.
+  reflexivity.
+
+Qed.
+*)
+
+Theorem splitmsb_ls_eq : forall n (b : spec.BITS (S n)),
+  splitmsb_ls (tuple.tval b)  = 
+    let p :=
+      (spec.splitmsb b) in (fst p, (tuple.tval (snd p))).
+
+  intros.
+  remember (spec.splitmsb b) as z.
+  destruct z.
+  symmetry in Heqz.
+  apply splitmsb_rev in Heqz.
+  simpl.
+  unfold splitmsb_ls.
+  rewrite Heqz.
+  rewrite seq.revK.
+  reflexivity.
+Qed.
+
+Theorem toZ_ls_eq : forall n (b : spec.BITS (S n)),
+  toZ_ls (tuple.tval b) = spec.toZ b.
+
+  intros.
+  unfold toZ_ls, spec.toZ.
+  rewrite splitmsb_ls_eq.
+  remember (spec.splitmsb b) as z.
+  destruct z.
+  simpl.
+  destruct b0.
+  reflexivity.
+  reflexivity.
+
+Qed.
+
+Theorem sbvToInt_ls_equiv : forall n (v : Vec n bool),
+  sbvToInt_ls v = sbvToInt n v.
+
+  intros.
+  destruct n; simpl in *; trivial.
+  rewrite <- toZ_ls_eq.
+  rewrite bvToBITS_ls_equiv.
+  reflexivity.
+
+Qed.
+
+Theorem seq_rev_eq : forall (A : Type)(ls : list A),
+  seq.rev ls = rev ls.
+
+  induction ls; intros; simpl in *; trivial.
+  rewrite <- IHls.
+  rewrite seq.rev_cons.
+  rewrite <- seq.cats1.
+  reflexivity.
+
+Qed.
+
+Theorem toNegZ_ls_nonneg : forall ls,
+  0 <= toNegZ_ls ls.
+
+  induction ls; intros; simpl in *.
+  lia.
+  destruct a; simpl in *; lia.
+
+Qed.
+
+Theorem nonneg_sign_bit_clear :  forall n v h,
+  0 <= sbvToInt (S n) (VectorDef.cons h v) ->
+  h = false.
+
+  intros. 
+  rewrite <- sbvToInt_ls_equiv in *.
+  simpl in *.
+  unfold bvToBITS_ls in *.
+  rewrite to_list_cons in H.
+  simpl in *.
+  
+  unfold toZ_ls in *.
+  unfold splitmsb_ls in *.
+  rewrite seq_rev_eq in *.
+  rewrite rev_app_distr in H.
+  rewrite rev_involutive in *.
+  simpl in *.
+  destruct h; simpl in *; trivial.
+  match goal with 
+  | [H: 0 <= - Z.succ (toNegZ_ls ?a) |- _] =>
+    remember a as z
+  end.
+  specialize (toNegZ_ls_nonneg z); intros.
+  lia.
+Qed.
+
+
+Theorem shiftR_all_nonneg : forall n1 v,
+  n1 <> O ->
+  (0 <= sbvToInt _ v)%Z ->
+  (shiftR n1 bool false v (pred n1)) = replicate n1 bool false.
+
+  intros.
+  apply eq_if_to_list_eq.
+  rewrite <- replicate_repeat_eq.
+  rewrite shiftR_ls_equiv.
+  rewrite shiftR_ls_eq_repeat.
+  match goal with 
+  | [|- context[ (?a - ?b)%nat]] =>
+  replace (a - b)%nat with 1%nat
+  end.
+  destruct v; simpl; trivial.
+  erewrite (nonneg_sign_bit_clear _ h); eauto.
+  replace [false] with (repeat false 1%nat); trivial.
+  rewrite <- repeat_app.
+  rewrite plus_comm.
+  trivial.
+  rewrite to_list_length.
+  lia.
+  rewrite to_list_length.
+  lia.
+
+Qed.
+
+Theorem neg_sign_bit_set :  forall n v h,
+  sbvToInt (S n) (VectorDef.cons h v) < 0 ->
+  h = true.
 
 Admitted.
+
+Definition zero_ls n := repeat false n.
+
+
+Fixpoint fromPosZ_ls n z :=
+  match n with
+    | 0%nat => nil
+    | S n0 => joinlsb_ls (fromPosZ_ls n0 (Z.div2 z), negb (Z.even z))
+  end.
+
+Fixpoint fromNegZ_ls n z :=
+  match n with
+    | 0%nat => nil
+    | S n0 => joinlsb_ls (fromNegZ_ls n0 (Z.div2 z), Z.even z)
+  end.
+
+Definition fromZ_ls n z :=
+  match z with
+     | 0 => zero_ls n
+     | Z.pos _ => fromPosZ_ls n z
+     | Z.neg _ => fromNegZ_ls n (Z.pred (- z))
+   end.
+
+
+Definition bitsToBv_ls (ls : list bool) := rev ls.
+
+Definition bitsToBv_ls_0 size := 
+tuple_foldl_dep bool (fun n : Nat => list bool) size
+  (fun (n : Nat) ls (b : bool) => b::ls) (@nil bool).
+
+Theorem tuple_S_ex : forall (A : Type) n (t : tuple.tuple_of (S n) A),
+  exists a (t' : tuple.tuple_of n A),
+  t = tuple.cons_tuple a t'.
+
+  intros.
+  exists (tuple.thead t).
+  exists (tuple.behead_tuple t).
+  apply tuple.tuple_eta.
+
+Qed.
+
+Theorem tuple_head_cons : forall (A: Type) n x (x0 : tuple.tuple_of n A),
+  (tuple.thead (tuple.cons_tuple x x0)) = x.
+
+  intros.
+  apply tuple.theadCons.
+
+Qed.
+
+Theorem tuple_behead_cons : forall (A: Type) n x (x0 : tuple.tuple_of n A),
+  (tuple.behead_tuple (tuple.cons_tuple x x0)) = x0.
+
+  intros.
+  apply tuple.beheadCons.
+
+Qed.
+
+Theorem tuple_tval_cons : forall (A: Type) n x (x0 : tuple.tuple_of n A),
+  (tuple.tval (tuple.cons_tuple x x0)) = x :: (tuple.tval x0).
+
+  intros.
+  reflexivity.
+
+Qed.
+
+Theorem tuple_foldl_dep_conv_const_equiv : forall (A : Type) n (v : tuple.tuple_of n A)
+  (B1 : nat -> Type)(B2 : Type)
+  (conv : forall n, B1 n -> B2) b1
+  (f1 : forall (n : nat), B1 n -> A -> B1 (S n))(f2 : B2 -> A -> B2),
+  (forall n b a, conv _ (f1 n b a) = f2 (conv _ b) a) ->
+  conv _ (tuple_foldl_dep A B1 n f1 b1 v) = tuple_foldl_dep A (fun _ => B2) n (fun _ => f2) (conv _ b1) v.
+
+  induction n; intros; simpl in *; trivial.
+  destruct (tuple_S_ex v).
+  destruct H0.
+  subst.
+  
+  specialize (IHn x0).
+  specialize (IHn (fun n => B1 (S n)) B2).
+  specialize (IHn (fun n => conv (S n))).
+  specialize (IHn (f1 _ b1 x)).
+  
+  specialize (IHn (fun n0 : nat => f1 (S n0)) f2).
+  simpl in *.
+  unfold Nat in *.
+  rewrite tuple_head_cons.
+  rewrite tuple_behead_cons.
+  rewrite IHn.
+  rewrite H.
+  reflexivity.
+
+  intros.
+  eapply H.
+
+Qed.
+
+Theorem tuple_fold_dep_ls_equiv : forall (A : Type) n (v : tuple.tuple_of n A)
+  (B : Type)(f : B -> A -> B) b,
+  tuple_foldl_dep A (fun _ => B) n (fun _ => f) b v = fold_left f (tuple.tval v) b.
+
+  induction n; intros.
+  simpl in *.
+  destruct v.
+  destruct tval; simpl in *; trivial.
+  inversion i.
+
+  destruct (tuple_S_ex v).
+  destruct H.
+  subst.
+  simpl.
+  rewrite tuple_behead_cons.
+  rewrite tuple_head_cons.
+  rewrite IHn.
+  reflexivity.
+
+Qed.
+
+Theorem bitsToBv_ls_0_eq : forall n (bs : spec.BITS n),
+  bitsToBv_ls_0 bs = to_list (bitsToBv bs).
+
+  intros.
+  symmetry.
+  unfold bitsToBv_ls_0, bitsToBv.
+  specialize (tuple_foldl_dep_conv_const_equiv bs (Vector.t bool) (@to_list bool)); intros.
+  simpl in *.
+  erewrite H.
+  replace (to_list (Vector.nil Bool)) with (@nil bool).
+  reflexivity.
+  reflexivity.
+  intros. simpl.
+  rewrite to_list_cons.
+  reflexivity.
+
+Qed.
+
+Theorem bitsToBv_ls_eq : forall n (bs : spec.BITS n),
+  bitsToBv_ls (tuple.tval bs) = to_list (bitsToBv bs).
+
+  intros.
+  rewrite <- bitsToBv_ls_0_eq.
+
+  unfold bitsToBv_ls_0, bitsToBv_ls.
+  rewrite tuple_fold_dep_ls_equiv.
+  generalize (tuple.tval bs) as ls.
+  induction ls using rev_ind; intros; simpl in *; trivial.
+  rewrite rev_app_distr.
+  simpl.
+  rewrite IHls.
+  rewrite fold_left_app.
+  simpl.
+  reflexivity.
+
+Qed.
+
+Definition intToBv_ls n z:=
+  bitsToBv_ls (fromZ_ls n z).
+
+
+Theorem tuple_nseq_ls_eq : forall n (A : Type) (a: A), 
+  repeat a n = tuple.tval (tuple.nseq_tuple n a).
+
+  induction n; intros; simpl in *; trivial.
+
+  f_equal; eauto.
+
+Qed.
+
+Theorem zero_ls_eq : forall n,
+  zero_ls n = tuple.tval (spec.zero n).
+
+  intros.
+  eapply tuple_nseq_ls_eq.
+Qed.
+
+Theorem fromPosZ_ls_eq : forall n z,
+  fromPosZ_ls n z = tuple.tval (@spec.fromPosZ n z).
+
+  induction n; intros; simpl in *; trivial.
+  unfold joinlsb_ls.
+  simpl.
+  f_equal.
+  eauto.
+
+Qed.
+
+Theorem fromNegZ_ls_eq : forall n z,
+  fromNegZ_ls n z = tuple.tval (@spec.fromNegZ n z).
+
+  induction n; intros; simpl in *; trivial.
+  unfold joinlsb_ls.
+  simpl.
+  f_equal.
+  eauto.
+
+Qed.
+
+Theorem fromZ_ls_eq : forall n z,
+  fromZ_ls n z = tuple.tval (@spec.fromZ n z).
+
+  intros.
+  unfold fromZ_ls, spec.fromZ.
+  destruct z.
+  apply zero_ls_eq.
+  apply fromPosZ_ls_eq.
+  apply fromNegZ_ls_eq.
+
+Qed.
+
+Theorem intToBv_ls_eq : forall n z,
+  intToBv_ls n z = to_list (intToBv n z).
+
+  intros.
+  unfold intToBv, intToBv_ls.
+  rewrite <- bitsToBv_ls_eq.
+  f_equal.
+  apply fromZ_ls_eq.
+
+Qed.
+
+Theorem fromPosZ_ls_0_eq : forall n,
+  fromPosZ_ls n 0 = repeat 0%bool n.
+
+  induction n; intros; simpl in *; trivial.
+  unfold joinlsb_ls.
+  simpl.
+  f_equal.
+  eauto.
+
+Qed.
+
+Theorem fromZ_ls_1_eq :  forall n,
+  fromZ_ls (S n) 1 = true :: repeat false n.
+
+  intros.
+  unfold fromZ_ls.
+  simpl.
+  unfold joinlsb_ls.
+  simpl.
+  f_equal.
+  apply fromPosZ_ls_0_eq.
+
+Qed.
+
+Theorem repeat_S_rev : forall (A : Type) n (a : A),
+  repeat a (S n) = (repeat a n) ++ [a].
+
+  induction n; intros; simpl in *; trivial.
+  f_equal.
+  eauto.
+
+Qed.
+
+Theorem rev_repeat_id : forall (A : Type) n (a : A),
+  rev (repeat a n) = repeat a n.
+
+  induction n; intros; simpl in *; trivial.
+  rewrite IHn.
+  destruct n.
+  simpl in *; trivial.
+  rewrite repeat_S_rev at 2.
+  simpl.
+  reflexivity.
+
+Qed.
+
+Theorem intToBv_1_to_list_eq : forall n, 
+  to_list (intToBv (S n) 1) = repeat 0%bool n ++ [true].
+
+  intros.
+  rewrite <- intToBv_ls_eq.
+  unfold intToBv_ls.
+  unfold bitsToBv_ls.
+  rewrite fromZ_ls_1_eq.
+  simpl.
+  rewrite rev_repeat_id.
+  reflexivity.
+
+Qed.
+
+Theorem shiftR_all_neg : forall n1 v,
+  n1 <> O ->
+  (sbvToInt _ v < 0)%Z ->
+  (shiftR n1 bool false v (pred n1)) = intToBv _ 1.
+
+  intros.
+  apply eq_if_to_list_eq.
+  rewrite shiftR_ls_equiv.
+  destruct v; simpl; trivial.
+  rewrite intToBv_1_to_list_eq.  
+  rewrite shiftR_ls_eq_repeat.
+  match goal with 
+  | [|- context[ (?a - ?b)%nat]] =>
+  replace (a - b)%nat with 1%nat
+  end.
+ 
+  erewrite (neg_sign_bit_set _ h); eauto.
+  rewrite to_list_length.
+  lia.
+  rewrite to_list_length.
+  lia.
+
+Qed.
+
+Theorem intToBv_0_eq_replicate : forall n,
+    intToBv n 0 = replicate n bool false.
+
+  intros.
+  apply eq_if_to_list_eq.
+  rewrite <- intToBv_ls_eq.
+  unfold intToBv_ls.
+  simpl.
+  unfold bitsToBv_ls, zero_ls.
+  rewrite rev_repeat_id.
+  rewrite replicate_repeat_eq.
+  reflexivity.
+
+Qed.
+
+
+Definition shiftin_ls(A : Type) a (ls : list A) :=
+  ls ++ [a].
+
+Definition shiftL1_ls (A : Type) (a : A) (ls : list A) :=
+  tl (shiftin_ls a ls).
+
+Definition shiftL_ls (A : Type) (x : A) (v : list A) (i : nat) := ssrnat.iter i (shiftL1_ls x) v.
+
+Theorem to_list_tl_eq : forall (A : Type) n (ls : Vec (S n) A),
+  to_list (Vector.tl ls) = tl (to_list ls).
+
+  intros.
+  destruct (Vec_S_cons ls).
+  destruct H.
+  subst.
+  reflexivity.
+
+Qed.
+
+Theorem shiftin_ls_eq : forall n (A : Type) a (ls : Vec n A),
+  to_list (shiftin a ls) = shiftin_ls a (to_list ls).
+
+  intros.
+  induction ls; intros; simpl in *.
+  rewrite to_list_cons.
+  reflexivity.
+
+  rewrite to_list_cons.
+  rewrite IHls.
+  unfold shiftin_ls.
+  rewrite to_list_cons.
+  rewrite app_comm_cons.
+  reflexivity.
+
+Qed.
+
+Theorem shiftL1_ls_eq : forall n (A : Type) a (ls : Vec n A),
+  to_list (shiftL1 n A a ls) = shiftL1_ls a (to_list ls).
+
+  intros.
+  unfold shiftL1, shiftL1_ls.
+  rewrite to_list_tl_eq.
+  f_equal.
+  apply shiftin_ls_eq.
+  
+Qed.
+
+
+Theorem shiftL_to_list_eq : forall n n1 (A : Type)(a : A)(ls : Vec n A),
+  to_list (shiftL n A a ls n1) = shiftL_ls a (to_list ls) n1.
+
+  induction n1; intros; simpl in *; trivial.
+  rewrite shiftL1_ls_eq.
+  f_equal.
+  eapply IHn1.
+
+Qed.
+
+(*
+
+Theorem rev_shiftL_ls_eq_h : forall (A : Type) n1 n2 n (a b : A),
+  (n < n1)%nat ->
+  rev (shiftL_ls a (repeat a n1 ++ [b] ++ repeat a n2) n) = shiftR_ls a (repeat a n2 ++ b:: (repeat a n1))  n.
+
+  induction n; intros; simpl in *.
+  rewrite rev_app_distr.
+  simpl.
+  rewrite <- app_assoc.
+  simpl.
+  repeat rewrite rev_repeat_id.
+  reflexivity.
+
+  
+
+  Search repeat rev.
+  rewrite repeat_rev_eq.
+  reflexivity.
+
+Qed.
+
 *)
+
+
+(*
+
+Theorem toZ_ls_shiftR_ls_eq_h : forall s n1 n2 a b,
+  (s < n2)%nat -> 
+  toZ_ls (shiftR_ls a (repeat a n1 ++ b :: repeat a n2) s) =  Z.shiftl (toZ_ls (repeat a n1 ++ b :: repeat a n2)) (Z.of_nat s).
+
+  induction s; intros.
+  simpl in *.
+  reflexivity.
+
+  rewrite Znat.Nat2Z.inj_succ.
+  rewrite <- Z.add_1_r.
+  rewrite <- (Z.shiftl_shiftl _ (Z.of_nat s) 1).
+  rewrite <- IHs.
+  simpl.
+  Search Z.shiftl.
+
+  Search toZ_ls shiftR1_ls.
+  
+
+Qed.
+*)
+
+Theorem shiftR1_ls_comm: forall (A : Type) (a : A) ls n1,
+  shiftR1_ls a (shiftR_ls a ls n1) = shiftR_ls a (shiftR1_ls a ls) n1.
+
+  induction n1; intros; simpl in *; trivial.
+  rewrite IHn1.
+  reflexivity.
+
+Qed.
+
+Theorem shiftR1_app_repeat_eq : forall n1 (A : Type)(a b : A) ls,
+  (n1 > 0)%nat ->
+  shiftR1_ls a (ls ++ repeat b n1) = (a :: ls ++ repeat b (pred n1)).
+
+  intros.
+  unfold shiftR1_ls, shiftout_ls.
+  simpl.
+  rewrite app_length. 
+
+  destruct n1.
+  simpl in *; lia.
+
+  rewrite repeat_S_rev at 2.
+  simpl.
+  rewrite plus_comm.
+  simpl.
+  f_equal.
+  rewrite plus_comm.
+  rewrite app_assoc.
+  rewrite firstn_app_1.
+  rewrite <- app_length.
+  apply firstn_all.
+  rewrite app_length.
+  lia.
+
+Qed.
+
+Theorem shiftout_ls_app_rev : forall (A : Type)(ls : list A) a,
+  shiftout_ls (ls ++ [a]) = ls.
+
+  intros.
+  unfold shiftout_ls.
+  rewrite app_length.
+  rewrite plus_comm.
+  simpl.
+  rewrite firstn_app_1.
+  apply firstn_all.
+  lia.
+
+Qed.
+
+Theorem splitmsb_ls_app_eq : forall ls a,
+  splitmsb_ls (ls ++ [a])  = (a, ls).
+
+  intros.
+  unfold splitmsb_ls.
+  rewrite seq_rev_eq.
+  rewrite rev_app_distr.
+  simpl.
+  rewrite seq_rev_eq.
+  rewrite rev_involutive.
+  reflexivity.
+
+Qed.
+
+Theorem toPosZ_app_0_eq : forall ls,
+  toPosZ_ls (ls ++ [0%bool]) = toPosZ_ls ls.
+
+  induction ls; intros; simpl in *; trivial.
+  destruct a.
+  rewrite IHls.
+  reflexivity.
+  rewrite IHls.
+  reflexivity.
+
+Qed.
+
+Theorem toPosZ_app_repeat_0_eq : forall n ls,
+  toPosZ_ls (ls ++ (repeat false n)) = toPosZ_ls ls.
+
+  induction n; intros; simpl in *.
+  rewrite app_nil_r.
+  reflexivity.
+  replace (ls ++ 0%bool :: repeat 0%bool n)  with ((ls ++ [false]) ++ repeat 0%bool n).
+  rewrite IHn.
+  apply toPosZ_app_0_eq.
+  rewrite <-  app_assoc.
+  reflexivity.
+
+Qed.
+
+
+Theorem toPosZ_cons_0_eq : forall ls,
+  toPosZ_ls (0%bool :: ls) = Z.double (toPosZ_ls ls).
+
+  reflexivity.
+Qed.
+
+Theorem toZ_ls_shiftR1_ls_eq : forall ls,
+  (length ls > 1)%nat ->
+  last ls false = false ->
+  last (removelast ls) false = false ->
+  toZ_ls (shiftR1_ls false ls) = Z.shiftl (toZ_ls ls ) 1.
+
+  destruct ls using rev_ind; intros; simpl in *.
+  unfold shiftR1_ls, shiftout_ls.
+  simpl.
+  reflexivity.
+
+  rewrite last_last in H0.
+  subst.
+
+  unfold shiftR1_ls.
+  rewrite (app_comm_cons).
+  rewrite shiftout_ls_app_rev.
+  unfold toZ_ls.
+  rewrite splitmsb_ls_app_eq.
+  
+  destruct ls using rev_ind.
+  simpl in *.
+  lia.
+
+  rewrite app_comm_cons.
+  rewrite splitmsb_ls_app_eq.
+  rewrite removelast_last in H1.
+  rewrite last_last in H1.
+  subst.
+  rewrite toPosZ_app_0_eq.
+  rewrite toPosZ_cons_0_eq.
+  remember (toPosZ_ls ls) as z.
+
+  destruct z;
+  lia.
+
+Qed.
+
+Theorem last_app_2 : forall (A : Type)(ls1 ls2 : list A) a,
+  (length ls2 > 0)%nat ->
+  last (ls1 ++ ls2) a = last ls2 a.
+
+
+  intros.
+  destruct ls2 using rev_ind.
+  simpl in *.
+  lia.
+
+  rewrite app_assoc.
+  rewrite last_last.
+  rewrite last_last.
+  reflexivity.
+
+Qed.
+
+Theorem last_repeat_eq : forall n (A : Type) (a : A),
+  last (repeat a n) a = a.
+
+  induction n; intros; simpl in *.
+  trivial.
+  rewrite IHn.
+  destruct (repeat a n); trivial.
+
+Qed.
+
+
+Theorem removelast_repeat_eq : forall (A : Type)(a : A) n,
+  (n > 0)%nat ->
+  removelast (repeat a n) = repeat a (pred n).
+
+  intros.
+  destruct n.
+  lia.
+  rewrite repeat_S_rev.
+  rewrite removelast_last.
+  reflexivity.
+
+Qed.
+
+Theorem removelast_length : forall (A : Type)(ls : list A),
+  ls <> nil ->
+  List.length (removelast ls) = pred (List.length ls).
+
+  induction ls using rev_ind; intros.
+  intuition idtac.
+  rewrite removelast_last.
+  rewrite app_length.
+  rewrite plus_comm.
+  simpl.
+  reflexivity.
+
+Qed.
+
+Theorem toZ_ls_shiftR_ls_eq : forall n n1 ls,
+  (n < n1)%nat ->
+  toZ_ls (shiftR_ls false (ls ++ repeat false n1) n) = Z.shiftl (toZ_ls (ls ++ repeat false n1) ) (Z.of_nat n).
+
+  induction n; intros.
+  simpl in *; trivial.
+
+  rewrite Znat.Nat2Z.inj_succ.
+  rewrite <- Z.add_1_l.
+
+  simpl.
+  rewrite shiftR1_ls_comm.
+  rewrite shiftR1_app_repeat_eq.
+  rewrite app_comm_cons.
+  rewrite IHn; try lia.
+
+  rewrite <- (Z.shiftl_shiftl _ 1 (Z.of_nat n)).
+  f_equal.
+  rewrite <- app_comm_cons.
+  rewrite <- shiftR1_app_repeat_eq; try lia.
+  rewrite toZ_ls_shiftR1_ls_eq.
+  reflexivity.
+
+  rewrite app_length.
+  rewrite repeat_length.
+  lia.
+  rewrite last_app_2.
+  apply last_repeat_eq.
+  rewrite repeat_length.
+  lia.
+  rewrite removelast_app.
+  rewrite last_app_2.
+  rewrite removelast_repeat_eq; try lia.
+  rewrite last_repeat_eq.
+  trivial.
+  rewrite removelast_length.
+  rewrite repeat_length.
+  lia.
+  intuition idtac.
+  apply length_zero_iff_nil in H0.
+  rewrite repeat_length in *.
+  lia.
+  intuition idtac.
+  apply length_zero_iff_nil in H0.
+  rewrite repeat_length in *.
+  lia.
+  lia.
+  lia.
+
+Qed.
+
+Theorem shiftL1_ls_shiftL_ls_comm : forall (A : Type) n (a : A) ls,
+  shiftL1_ls a (shiftL_ls a ls n) = shiftL_ls a (shiftL1_ls a ls) n.
+
+  induction n; intros; simpl in *; trivial.
+  rewrite IHn.
+  reflexivity.
+
+Qed.
+
+Theorem shiftL1_ls_repeat_eq : forall n1 (A : Type)(a : A) b,
+  (n1 > 0)%nat ->
+  (shiftL1_ls a (repeat a n1 ++ b)) = (repeat a (pred n1) ++ b ++ [a]).
+
+  intros.
+  unfold shiftL1_ls.
+  unfold shiftin_ls.
+  destruct n1; simpl in *; try lia.
+  rewrite app_assoc.
+  reflexivity.
+
+Qed.
+
+
+Theorem rev_shiftL_ls_eq_h : forall (A : Type) n n1 (a : A) b,
+  (n < n1)%nat ->
+  rev (shiftL_ls a (repeat a n1 ++ b ) n) = shiftR_ls a ((rev b)++ (repeat a n1))  n.
+
+  induction n;
+  intros;
+  simpl in *.
+  rewrite rev_app_distr.
+  rewrite rev_repeat_id.
+  reflexivity.
+
+  rewrite shiftL1_ls_shiftL_ls_comm.
+  rewrite shiftL1_ls_repeat_eq.
+  rewrite IHn.
+  rewrite shiftR1_ls_comm.
+  rewrite shiftR1_app_repeat_eq.
+  rewrite rev_app_distr.
+  simpl.
+  reflexivity.
+  lia.
+  lia.
+  lia.
+
+Qed.
+
+
+Theorem rev_shiftL_ls_eq : forall (A : Type) n1 n (a b : A),
+  (n < n1)%nat ->
+  rev (shiftL_ls a (repeat a n1 ++ [b] ) n) = shiftR_ls a (b:: (repeat a n1))  n.
+
+  intros.
+  apply rev_shiftL_ls_eq_h.
+  trivial.
+
+Qed.
+
+Theorem sbvToInt_shiftL_1_equiv : forall n s,
+  (n > 0)%nat ->
+  (s < pred n)%nat ->
+  sbvToInt n (shiftL _ _ false (intToBv _ 1) s) = 
+  Z.shiftl 1 (Z.of_nat s).
+
+  intros.
+  rewrite <- sbvToInt_ls_equiv.
+  unfold sbvToInt_ls.
+  destruct n.
+  lia.
+  unfold bvToBITS_ls.
+  rewrite shiftL_to_list_eq.
+  rewrite <- intToBv_ls_eq.
+  unfold intToBv_ls, bitsToBv_ls.
+  simpl in *.
+  rewrite fromPosZ_ls_0_eq.
+  rewrite rev_repeat_id.
+  rewrite rev_shiftL_ls_eq.
+  replace (1%bool :: repeat 0%bool n) with ([true] ++ (repeat false n)).
+  rewrite toZ_ls_shiftR_ls_eq.
+  unfold toZ_ls.
+  Search splitmsb_ls app.
+  destruct n.
+  lia.
+  rewrite repeat_S_rev.
+  rewrite app_assoc.
+  Search splitmsb_ls app.
+  rewrite splitmsb_ls_app_eq.
+  
+  rewrite toPosZ_app_repeat_0_eq.
+  simpl.
+  reflexivity.
+  lia.
+  simpl.
+  reflexivity.
+  lia.
+
+Qed.
+
+Theorem toPosZ_ls_repeat_0 : forall n,
+  toPosZ_ls (repeat 0%bool n) = 0.
+
+  induction n; intros; simpl in *; trivial.
+  rewrite IHn.
+  lia.
+
+Qed.
+
+Theorem sbvToInt_replicate_0 : forall n,
+  sbvToInt _ (replicate n bool false) = 0.
+
+  intros.
+  rewrite <- sbvToInt_ls_equiv.
+  unfold sbvToInt_ls.
+  destruct n; simpl; trivial.
+  unfold bvToBITS_ls.
+  rewrite <- replicate_repeat_eq.
+  rewrite rev_repeat_id.
+  rewrite repeat_S_rev.
+  unfold toZ_ls.
+  rewrite splitmsb_ls_app_eq.
+  apply toPosZ_ls_repeat_0.
+  
+Qed.
+
+Theorem nth_to_list_eq : forall (A : Type) n (f : Fin.t n) (v : Vec n A) a,
+  Vector.nth v f = nth (proj1_sig (Fin.to_nat f) ) (to_list v) a.
+
+  induction f; intros; simpl in *; subst.
+  destruct (Vec_S_cons v).
+  destruct H. 
+  subst.
+  rewrite to_list_cons.
+  simpl.
+  reflexivity.
+
+  remember (Fin.to_nat f ) as z.  
+  destruct z.
+  simpl.
+  
+  destruct (Vec_S_cons v).
+  destruct H. 
+  subst.
+  rewrite to_list_cons.
+  simpl in *.
+  eapply IHf.
+
+Qed.
+
+Theorem nth_to_list_eq_gen : forall (A : Type) n (f : Fin.t n) (v : Vec n A) a n',
+  n' = (proj1_sig (Fin.to_nat f) ) ->
+  Vector.nth v f = nth n' (to_list v) a.
+
+  intros.
+  subst.
+  apply nth_to_list_eq. 
+
+Qed.
+
+
+Theorem nth_order_to_list_eq : forall (A : Type) (a : A) n (v : Vec n A) n' (pf : (n' < n)%nat),
+  nth_order v pf = nth n' (to_list v) a.
+
+  intros.
+  unfold nth_order.
+  eapply nth_to_list_eq_gen.
+  rewrite Fin.to_nat_of_nat.
+  reflexivity.
+
+Qed.
+
+Theorem toPosZ_ls_nonneg : forall ls,
+  0 <= toPosZ_ls ls.
+
+  induction ls; intros; simpl in *; try lia.
+  destruct a; lia.
+
+Qed.
+
+Theorem toPosZ_ls_In_true_nz : forall ls,
+  In true ls ->
+  toPosZ_ls ls <> 0%Z.
+
+  induction ls; intros; simpl in *.
+  intuition idtac.
+  destruct H.
+  subst.
+  specialize (toPosZ_ls_nonneg ls); intros.
+  lia.
+  destruct a.
+  specialize (toPosZ_ls_nonneg ls); intros.
+  lia.
+  intuition idtac.
+  lia.
+Qed.
+
+Theorem toZ_ls_In_true_nz : forall ls,
+  In true ls ->
+  toZ_ls ls <> 0%Z.
+
+  intros.
+  destruct ls using rev_ind; intros; simpl in *.
+  intuition idtac.
+  unfold toZ_ls.
+  rewrite splitmsb_ls_app_eq.
+  apply in_app_or in H.
+
+  destruct x.
+  specialize (toNegZ_ls_nonneg ls); intros.
+  lia.
+
+  destruct H.
+  eapply toPosZ_ls_In_true_nz; eauto.
+
+  simpl in *.
+  intuition idtac.
+  discriminate.
+
+Qed.
+
+Theorem sbvToInt_nz_nth : forall n (v : Vec n _) n' (nlt : (n' < n)%nat),
+  nth_order v nlt = true ->
+  sbvToInt _ v <> 0%Z.
+
+  intros.
+  rewrite <- sbvToInt_ls_equiv.
+  unfold sbvToInt_ls.
+  destruct n.
+  lia.
+  
+  unfold bvToBITS_ls.
+  rewrite (@nth_order_to_list_eq _ false) in H.
+  assert (In true (to_list v)).
+  rewrite <- H.
+  apply nth_In.
+  rewrite to_list_length.
+  trivial.
+  apply toZ_ls_In_true_nz.
+  apply (@in_rev _ (to_list v)).
+  trivial.
+
+Qed.
+
+Theorem sbvToInt_neg_sign_bit_set : forall n  b2 (ltpf : (0 < n)%nat),
+    (sbvToInt n b2 < 0)%Z ->
+    nth_order b2 ltpf = true.
+
+  intros.
+  rewrite <- sbvToInt_ls_equiv in *.
+  unfold sbvToInt_ls in *.
+  destruct n.
+  lia.
+  unfold bvToBITS_ls in *.
+  destruct (Vec_S_cons b2).
+  destruct H0.
+  subst.
+  rewrite to_list_cons in *.
+  unfold toZ_ls in *.
+  simpl in *.
+  rewrite splitmsb_ls_app_eq in *.
+  destruct x.
+  reflexivity.
+  match goal with
+  | [H : toPosZ_ls ?a < 0 |- _ ] =>
+    specialize (toPosZ_ls_nonneg a); intros
+  end.
+  lia.
+
+Qed.
+
+Theorem toZ_ls_repeat_0: forall n : nat, 
+  toZ_ls (repeat 0%bool n) = 0.
+
+  intros.
+  unfold toZ_ls.
+  destruct n.
+  simpl.
+  reflexivity.
+
+  rewrite repeat_S_rev.
+  rewrite splitmsb_ls_app_eq.
+  apply toPosZ_ls_repeat_0.
+
+Qed.
+
+Theorem splitmsb_ls_eq_app_if : forall ls a ls',
+  (ls <> nil) ->
+  splitmsb_ls ls = (a, ls') ->
+  ls = ls' ++ [a].
+
+  intros.
+  destruct ls using rev_ind.
+  intuition idtac.
+
+  rewrite splitmsb_ls_app_eq in H0.
+  inversion H0; clear H0; subst.
+  reflexivity.
+
+Qed.
+
+Theorem Z_div_mul_eq : forall x y,
+  x > 0 ->
+  x * (y / x) = y - (y mod x).
+
+  intros.
+  specialize (Zdiv.Z_div_mod_eq y x); intuition idtac.
+  lia.
+
+Qed.
+
+Theorem Z_mod_div_eq : forall x y z,
+  z > 0 ->
+  y > 0 ->
+  y mod z = 0 ->
+  Z.div (Z.modulo x y) z = Z.modulo (Z.div x z) (Z.div y z).
+
+  intros.
+  assert (exists y', y = y'*z).
+  exists (y / z).
+  rewrite (@Zdiv.Z_div_exact_full_2 y z); trivial; try lia.
+  rewrite Z.mul_comm.
+  rewrite Z.div_mul.
+  reflexivity.
+  lia.
+  destruct H2.
+  subst.
+
+  destruct (Z.eq_decidable x0 0).
+  subst.
+  repeat rewrite Z.mul_0_l.
+  repeat rewrite Z.div_0_l.
+  repeat rewrite Zdiv.Zmod_0_r.
+  apply Z.div_0_l.
+  lia.
+  lia.
+
+  rewrite Zdiv.Z_div_mult; try lia.
+  rewrite Z.mul_comm.
+  rewrite Z.rem_mul_r.
+  rewrite Z.mul_comm.
+  rewrite Zdiv.Z_div_plus.
+  rewrite Zdiv.Zmod_div.
+  lia.
+  lia.
+  lia.
+  lia.
+Qed.
+
+
+Theorem fromPosZ_ls_app : forall n1 n2 z, 
+ 
+  fromPosZ_ls (n1 + n2) z = (fromPosZ_ls n1 (Z.modulo z (Z.pow 2 (Z.of_nat n1)))) ++ (fromPosZ_ls n2 (Z.div z (Z.pow 2 (Z.of_nat n1)))). 
+
+  induction n1; intros.
+  simpl in *.
+  rewrite Z.div_1_r.
+  reflexivity.
+
+  rewrite Znat.Nat2Z.inj_succ.
+  rewrite <- Z.add_1_r.
+  simpl in *.
+  unfold joinlsb_ls.
+  simpl.
+  f_equal.
+  f_equal.
+  repeat rewrite Zdiv.Zeven_mod.
+  f_equal.
+  rewrite Z.pow_add_r.
+  rewrite Z.mul_comm.
+  rewrite Z.rem_mul_r.
+  rewrite <- Zdiv.Zplus_mod_idemp_r.
+  rewrite Z.mul_comm.
+  rewrite Zdiv.Z_mod_mult.
+  rewrite Z.add_0_r.  
+  rewrite Z.pow_1_r.
+  rewrite Z.mod_mod.
+  reflexivity.
+  lia.
+  lia.
+  apply Z.pow_pos_nonneg; lia.
+  lia.
+  lia.
+
+  rewrite IHn1.
+  repeat rewrite Z.div2_div.
+  f_equal.
+  f_equal.
+  replace (2 ^ (Z.of_nat n1 + 1)) with ((2 ^ (Z.of_nat n1))*2).
+  rewrite Z_mod_div_eq; try lia.
+  rewrite Zdiv.Z_div_mult.
+  reflexivity.
+  lia.
+  apply Zorder.Zmult_gt_0_compat.
+  apply Z.lt_gt.
+  apply Z.pow_pos_nonneg; lia.
+  lia.
+  apply Zdiv.Z_mod_mult.
+  rewrite Z.pow_add_r.
+  reflexivity.
+  lia.
+  lia.
+
+  f_equal.
+  rewrite Z.pow_add_r; try lia.
+  rewrite Z.mul_comm.
+  rewrite Zdiv.Zdiv_Zdiv; try lia.
+  reflexivity.
+  apply Z.pow_nonneg; lia.
+
+Qed.
+
+Theorem fromPosZ_ls_rev : forall n z, 
+  (n > 0)%nat ->
+  fromPosZ_ls n z = (fromPosZ_ls (pred n) (Z.modulo z (Z.pow 2 (Z.of_nat (pred n))))) ++ [negb (Z.even (Z.div z (Z.pow 2 (Z.of_nat (pred n)))))]. 
+
+  intros.
+  destruct n.
+  lia.
+
+  replace (S n) with (n + 1)%nat; try lia.
+  rewrite fromPosZ_ls_app.
+  rewrite plus_comm.
+  simpl.
+  reflexivity.
+
+Qed.
+
+Theorem toPosZ_ls_fromPosZ_ls_eq : forall n z,
+  0 <= z < 2^(Z.of_nat n) ->
+  toPosZ_ls (fromPosZ_ls n z) = z.
+
+  induction n; intros.
+  simpl in *.
+  lia.
+
+  rewrite Znat.Nat2Z.inj_succ in *.
+  rewrite <- Z.add_1_r in *.
+  simpl in *.
+  case_eq (Z.even z); intros; simpl in *.
+  assert (exists z', z = 2 * z').
+  exists (Z.div2 z).
+  rewrite Zeven.Zdiv2_odd_eqn at 1.
+  rewrite <- Z.negb_even.
+  rewrite H0.
+  simpl.
+  rewrite Z.add_0_r.
+  reflexivity.
+  destruct H1. subst.
+  rewrite Z.div2_div.
+  rewrite Z.mul_comm.
+  rewrite Zdiv.Z_div_mult; try lia.
+  rewrite Z.double_spec.
+  rewrite IHn.
+  lia.
+  intuition idtac.
+  lia.
+  rewrite Z.pow_add_r in H2.
+  rewrite Z.mul_comm in H2.
+  rewrite Z.pow_1_r in H2.
+  eapply Zorder.Zmult_lt_reg_r; eauto.
+  lia.
+  lia.
+  lia.
+
+  assert (exists z', z = 1 + z' *2 ).
+  exists (Z.div2 z).
+  rewrite Zeven.Zdiv2_odd_eqn at 1.
+  rewrite <- Z.negb_even.
+  rewrite H0.
+  unfold negb.
+  lia.
+
+  destruct H1. subst.
+  rewrite <- Z.add_1_l.
+  f_equal.
+  rewrite Z.div2_div.
+  rewrite Zdiv.Z_div_plus.
+  simpl.
+  rewrite IHn.
+  rewrite Z.double_spec.
+  lia.
+  intuition idtac.
+  lia.
+  rewrite Z.pow_add_r in H2.
+  rewrite Z.mul_comm in H2.
+  rewrite Z.pow_1_r in H2.
+  lia.
+  lia.
+  lia.
+  lia.
+Qed.
+
+Theorem fromNegZ_ls_app : forall n1 n2 z, 
+ 
+  fromNegZ_ls (n1 + n2) z = (fromNegZ_ls n1 (Z.modulo z (Z.pow 2 (Z.of_nat n1)))) ++ (fromNegZ_ls n2 (Z.div z (Z.pow 2 (Z.of_nat n1)))). 
+
+  induction n1; intros.
+  simpl in *.
+  rewrite Z.div_1_r.
+  reflexivity.
+
+  rewrite Znat.Nat2Z.inj_succ.
+  rewrite <- Z.add_1_r.
+  simpl in *.
+  unfold joinlsb_ls.
+  simpl.
+  f_equal.
+  repeat rewrite Zdiv.Zeven_mod.
+  f_equal.
+  rewrite Z.pow_add_r.
+  rewrite Z.mul_comm.
+  rewrite Z.rem_mul_r.
+  rewrite <- Zdiv.Zplus_mod_idemp_r.
+  rewrite Z.mul_comm.
+  rewrite Zdiv.Z_mod_mult.
+  rewrite Z.add_0_r.  
+  rewrite Z.pow_1_r.
+  rewrite Z.mod_mod.
+  reflexivity.
+  lia.
+  lia.
+  apply Z.pow_pos_nonneg; lia.
+  lia.
+  lia.
+
+  rewrite IHn1.
+  repeat rewrite Z.div2_div.
+  f_equal.
+  f_equal.
+  replace (2 ^ (Z.of_nat n1 + 1)) with ((2 ^ (Z.of_nat n1))*2).
+  rewrite Z_mod_div_eq; try lia.
+  rewrite Zdiv.Z_div_mult.
+  reflexivity.
+  lia.
+  apply Zorder.Zmult_gt_0_compat.
+  apply Z.lt_gt.
+  apply Z.pow_pos_nonneg; lia.
+  lia.
+  apply Zdiv.Z_mod_mult.
+  rewrite Z.pow_add_r.
+  reflexivity.
+  lia.
+  lia.
+
+  f_equal.
+  rewrite Z.pow_add_r; try lia.
+  rewrite Z.mul_comm.
+  rewrite Zdiv.Zdiv_Zdiv; try lia.
+  reflexivity.
+  apply Z.pow_nonneg; lia.
+
+Qed.
+
+
+Theorem fromNegZ_ls_rev : forall n z, 
+  (n > 0)%nat ->
+  fromNegZ_ls n z = (fromNegZ_ls (pred n) (Z.modulo z (Z.pow 2 (Z.of_nat (pred n))))) ++ [(Z.even (Z.div z (Z.pow 2 (Z.of_nat (pred n)))))]. 
+
+  intros.
+  destruct n.
+  lia.
+
+  replace (S n) with (n + 1)%nat; try lia.
+  rewrite fromNegZ_ls_app.
+  rewrite plus_comm.
+  simpl.
+  unfold joinlsb_ls. simpl.
+  reflexivity.
+
+Qed.
+
+Theorem toNegZ_ls_fromNegZ_ls_eq : forall n z,
+  0 <= z < 2^(Z.of_nat n) ->
+  toNegZ_ls (fromNegZ_ls n z) = z.
+
+  induction n; intros.
+  simpl in *.
+  lia.
+
+  rewrite Znat.Nat2Z.inj_succ in *.
+  rewrite <- Z.add_1_r in *.
+  simpl in *.
+  case_eq (Z.even z); intros; simpl in *.
+  assert (exists z', z = 2 * z').
+  exists (Z.div2 z).
+  rewrite Zeven.Zdiv2_odd_eqn at 1.
+  rewrite <- Z.negb_even.
+  rewrite H0.
+  simpl.
+  rewrite Z.add_0_r.
+  reflexivity.
+  destruct H1. subst.
+  rewrite Z.div2_div.
+  rewrite Z.mul_comm.
+  rewrite Zdiv.Z_div_mult; try lia.
+  rewrite Z.double_spec.
+  rewrite IHn.
+  lia.
+  intuition idtac.
+  lia.
+  rewrite Z.pow_add_r in H2.
+  rewrite Z.mul_comm in H2.
+  rewrite Z.pow_1_r in H2.
+  eapply Zorder.Zmult_lt_reg_r; eauto.
+  lia.
+  lia.
+  lia.
+
+  assert (exists z', z = 1 + z' *2 ).
+  exists (Z.div2 z).
+  rewrite Zeven.Zdiv2_odd_eqn at 1.
+  rewrite <- Z.negb_even.
+  rewrite H0.
+  unfold negb.
+  lia.
+
+  destruct H1. subst.
+  rewrite <- Z.add_1_l.
+  f_equal.
+  rewrite Z.div2_div.
+  rewrite Zdiv.Z_div_plus.
+  simpl.
+  rewrite IHn.
+  rewrite Z.double_spec.
+  lia.
+  intuition idtac.
+  lia.
+  rewrite Z.pow_add_r in H2.
+  rewrite Z.mul_comm in H2.
+  rewrite Z.pow_1_r in H2.
+  lia.
+  lia.
+  lia.
+  lia.
+Qed.
+
+
+Theorem sbvToInt_intToBv_id : forall n v,
+  (n > 0)%nat ->
+  (-Z.pow 2 (Z.of_nat (pred n)) <= v < Z.pow 2 (Z.of_nat (pred n)))%Z ->
+  sbvToInt n (intToBv n v) = v.
+
+  intros.
+  rewrite <- sbvToInt_ls_equiv .
+  unfold sbvToInt_ls .
+  destruct n.
+  lia.
+
+  unfold bvToBITS_ls.
+  rewrite <- intToBv_ls_eq.
+  unfold intToBv_ls, bitsToBv_ls.
+  rewrite rev_involutive.
+  simpl in *.
+  unfold fromZ_ls.
+  destruct v.
+  unfold zero_ls.
+  apply toZ_ls_repeat_0.
+
+  rewrite fromPosZ_ls_rev.
+  simpl.
+  unfold toZ_ls.
+  rewrite splitmsb_ls_app_eq.
+  case_eq (Z.even (Z.pos p / 2^Z.of_nat n)); intros;
+  simpl.
+  rewrite Zdiv.Zmod_small.
+  apply toPosZ_ls_fromPosZ_ls_eq; intuition idtac; lia.
+  lia.
+  rewrite Z.div_small in H1.
+  simpl in *.
+  discriminate.
+  lia.
+  lia.
+
+  rewrite Pos2Z.opp_neg.
+  rewrite fromNegZ_ls_rev.
+  unfold pred.
+  unfold toZ_ls.
+  rewrite splitmsb_ls_app_eq.
+  case_eq (Z.even (Z.pred (Z.pos p) / 2^Z.of_nat n)); intros.
+  rewrite toNegZ_ls_fromNegZ_ls_eq.
+  rewrite Zdiv.Zmod_small.
+  lia.
+  lia.
+  apply Z.mod_bound_pos.
+  lia.
+  apply Z.pow_pos_nonneg; lia.
+  rewrite Z.div_small in H1.
+  simpl in *.
+  discriminate.
+  lia.
+  lia.
+Qed.
+
+
+
+
